backend/Inliningproof.v
@@ -1070,7 +1070,7 @@ Proof.
   intros. inv SIZES.
   destruct n; simpl in *. inv H0.
   econstructor; simpl; auto. etransitivity. apply H1.
-  simpl. generalize (Memory.frame_size_pos fr). intro. lia.
+  simpl. generalize (Memory.frame_size_a_pos fr). intro. lia.
   econstructor; simpl; eauto.
 Qed.
 
