x86/AsmFacts.v
@@ -1,0 +1,240 @@
+Require Import Coqlib Coqlib Maps.
+Require Import AST Integers Floats Values Memory Events Globalenvs Smallstep.
+Require Import Asm Asmgenproof0.
+
+(** instructions which have no relationship with stack *)
+Definition stk_unrelated_instr (i: instruction) :=
+  match i with
+    Pallocframe _ _ _
+  | Pfreeframe _ _ _
+  | Pcall_s _ _
+  | Pcall_r _ _
+  | Pret => false
+  | _ => true
+  end.
+
+(** modify RSP register *)
+(* Useful Lemmas *)
+Lemma nextinstr_rsp:
+  forall rs, nextinstr rs RSP = rs RSP.
+Proof.
+  unfold nextinstr.
+  intros; rewrite Pregmap.gso; congruence.
+Qed.
+
+Lemma nextinstr_nf_rsp:
+  forall rs, nextinstr_nf rs RSP = rs RSP.
+Proof.
+  unfold nextinstr_nf.
+  intros. rewrite nextinstr_rsp.
+  rewrite undef_regs_other; auto.
+  simpl; intuition subst; congruence.
+Qed.
+
+(* Internal Step *)
+(* Definition asm_exec_instr_unchange_rsp (i : instruction) : Prop := *)
+(*   forall ge rs1 m1 rs2 m2 f, *)
+(*     Asm.exec_instr ge f i rs1 m1 = Next rs2 m2 -> *)
+(*     rs2 # RSP = rs1 # RSP. *)
+
+Definition asm_instr_unchange_rsp (i : instruction) : Prop :=
+  forall ge f rs m rs' m',
+    stk_unrelated_instr i = true ->
+    Asm.exec_instr ge f i rs m = Next rs' m' ->
+    rs # RSP = rs' # RSP.
+
+(* Lemma find_instr_eq: *)
+(*   forall code ofs i, *)
+(*     find_instr ofs code = Some i -> In i code. *)
+(* Proof. *)
+(*   intro code. induction code. *)
+(*   - intros. inv H. *)
+(*   - intros. simpl in H. *)
+(*     destruct (zeq ofs 0) eqn:EQ. *)
+(*     + inv H. simpl. auto. *)
+(*     + apply IHcode in H. *)
+(*       simpl. right. auto. *)
+(* Qed. *)
+
+(* Definition asm_code_unchange_rsp (c : Asm.code) : Prop := *)
+(*   forall i, *)
+(*     In i c -> *)
+(*     asm_instr_unchange_rsp i. *)
+
+(* Definition asm_internal_unchange_rsp (ge: Genv.t Asm.fundef unit) : Prop := *)
+(*   forall b f, *)
+(*     Genv.find_funct_ptr ge b = Some (Internal f) -> *)
+(*     asm_code_unchange_rsp (fn_code f). *)
+
+Definition asm_internal_unchange_rsp (ge: Genv.t Asm.fundef unit) : Prop :=
+  forall b ofs f i,
+    Genv.find_funct_ptr ge b = Some (Internal f) ->
+    find_instr (Ptrofs.unsigned ofs) (fn_code f) = Some i ->
+    asm_instr_unchange_rsp i.
+
+(* Builtin Step *)
+Definition asm_builtin_unchange_rsp (ge: Genv.t Asm.fundef unit) : Prop :=
+  forall b ofs f ef args res (rs: regset) m vargs t vres rs' m',
+    Genv.find_funct_ptr ge b = Some (Internal f) ->
+    find_instr (Ptrofs.unsigned ofs) f.(fn_code) = Some (Pbuiltin ef args res) ->
+    eval_builtin_args ge rs (rs RSP) m args vargs ->
+    external_call ef ge vargs m t vres m' ->
+    rs' = nextinstr_nf
+              (set_res res vres
+                       (undef_regs (map preg_of (Machregs.destroyed_by_builtin ef)) rs)) ->
+    rs # RSP = rs' # RSP.
+
+(* Extenal Step *)
+Definition asm_external_unchange_rsp (ge: Genv.t Asm.fundef unit) : Prop :=
+  forall b ef args res rs m t rs' m',
+    Genv.find_funct_ptr ge b = Some (External ef) ->
+    extcall_arguments rs m (ef_sig ef) args ->
+    external_call ef ge args m t res m' ->
+    rs' = (set_pair (loc_external_result (ef_sig ef)) res (undef_caller_save_regs rs)) #PC <- (rs RA) ->
+    rs # RSP = rs' # RSP.
+
+Definition asm_prog_unchange_rsp (ge: Genv.t Asm.fundef unit) : Prop :=
+  asm_internal_unchange_rsp ge /\
+  asm_builtin_unchange_rsp ge /\
+  asm_external_unchange_rsp ge.
+
+(** Proof *)
+Definition no_rsp_pair (b: rpair preg) :=
+  match b with
+  | One r => r <> RSP
+  | Twolong hi lo => hi <> RSP /\ lo <> RSP
+  end.
+
+Lemma set_pair_no_rsp:
+  forall p res rs,
+    no_rsp_pair p ->
+    set_pair p res rs RSP = rs RSP.
+Proof.
+  destruct p; simpl; intros; rewrite ! Pregmap.gso; intuition.
+Qed.
+
+Lemma asm_external_unchange_rsp1 (ge: Genv.t Asm.fundef unit) :
+  asm_external_unchange_rsp ge.
+Proof.
+  red. intros.
+  subst.
+  assert (NORSPPAIR: no_rsp_pair (loc_external_result (ef_sig ef))).
+  {
+    red. unfold loc_external_result.
+    remember (Conventions1.loc_result (ef_sig ef)) as Mpair.
+    destruct Mpair; simpl.
+    - destruct r; try (simpl; congruence).
+    - split. destruct rhi; try (simpl; congruence).
+      destruct rlo; try (simpl; congruence).
+  }
+  repeat rewrite Pregmap.gso by (congruence).
+  rewrite set_pair_no_rsp; eauto.
+Qed.
+
+(** modify abstract stack *)
+Definition asm_instr_unchange_stk (i : instruction) : Prop :=
+  stk_unrelated_instr i = true ->
+  forall ge rs m rs' m' f,
+    Asm.exec_instr ge f i rs m = Next rs' m' ->
+    Mem.astack (Mem.support m) = Mem.astack (Mem.support m') /\
+    (forall b o k p, Mem.perm m b o k p <-> Mem.perm m' b o k p).
+
+
+Lemma exec_store_astack:
+    forall (ge: Genv.t Asm.fundef unit) k m1 a rs1 rs l rs2 m2,
+      exec_store ge k m2 a rs1 rs l = Next rs2 m1 ->
+      Mem.astack (Mem.support m2) = Mem.astack (Mem.support m1) /\ (forall b o k p, Mem.perm m2 b o k p <-> Mem.perm m1 b o k p).
+Proof.
+    intros ge k m1 a rs1 rs l rs2 m2  STORE.
+    unfold exec_store in STORE; repeat destr_in STORE.
+    unfold Mem.storev in Heqo; destr_in Heqo; inv Heqo.
+    erewrite <- Mem.support_store. 2: eauto.
+    split; auto.
+    split; intros.
+    eapply Mem.perm_store_1; eauto.
+    eapply Mem.perm_store_2; eauto.
+Qed.
+
+Lemma exec_load_astack:
+    forall (ge: Genv.t Asm.fundef unit) k m1 a rs1 rs rs2 m2,
+      exec_load ge k m2 a rs1 rs = Next rs2 m1 ->
+      Mem.astack (Mem.support m2) = Mem.astack (Mem.support m1) /\ (forall b o k p, Mem.perm m2 b o k p <-> Mem.perm m1 b o k p).
+Proof.
+    intros ge k m1 a rs1 rs rs2 m2 LOAD.
+    unfold exec_load in LOAD; destr_in LOAD.
+Qed.
+
+Lemma goto_label_astack:
+  forall (ge: Genv.t Asm.fundef unit) f l m1 rs1 rs2 m2,
+    goto_label ge f l rs1 m2 = Next rs2 m1 ->
+    Mem.astack (Mem.support m2) = Mem.astack (Mem.support m1) /\
+    (forall b o k p, Mem.perm m2 b o k p <-> Mem.perm m1 b o k p).
+Proof.
+    intros ge f l m1 rs1 rs2 m2 GOTO.
+    unfold goto_label in GOTO; repeat destr_in GOTO.
+Qed.
+
+Lemma asm_prog_unchange_stk (i : instruction) :
+  asm_instr_unchange_stk i.
+Proof.
+  intro.
+    intros ge0 rs1 m1 rs2 m2 f EI.
+      destruct i; simpl in H; try discriminate;
+        unfold exec_instr in EI; simpl in EI; repeat destr_in EI;
+          first [ split;[reflexivity|tauto]
+                | now (eapply exec_load_astack; eauto)
+                | now (eapply exec_store_astack; eauto)
+                | now ( eapply goto_label_astack; eauto)
+                | idtac ].
+    Unshelve. all: auto.
+    exact Mint32. exact PC.
+Qed.
+
+(** modify memory *)
+Lemma exec_store_unchange_support:
+  forall ge k a rs m r l rs' m',
+    Asm.exec_store ge k m a rs r l = Next rs' m' ->
+    Mem.sup_include (Mem.support m) (Mem.support m').
+Proof.
+  intros ge k a rs m r l rs' m' STORE.
+  unfold exec_store in STORE. repeat destr_in STORE.
+  apply Mem.support_storev in Heqo.
+  rewrite Heqo. apply Mem.sup_include_refl.
+Qed.
+
+Lemma exec_load_unchange_support:
+  forall ge k a m rs rd rs' m',
+    exec_load ge k m a rs rd = Next rs' m' ->
+    Mem.sup_include (Mem.support m) (Mem.support m').
+Proof.
+  intros ge k a m rs rd rs' m' LOAD.
+  unfold exec_load in LOAD. destr_in LOAD.
+Qed.
+
+Definition asm_instr_unchange_support (i : instruction) : Prop :=
+  forall ge rs m rs' m' f,
+    Asm.exec_instr ge f i rs m = Next rs' m' ->
+    Mem.sup_include (Mem.support m) (Mem.support m').
+
+Lemma asm_prog_unchange_support (i : instruction) :
+  asm_instr_unchange_support i.
+Proof.
+  red. intros *. intros EI. unfold exec_instr in EI.
+  destruct i; simpl in EI; inv EI; try (apply Mem.sup_include_refl);
+      first [ now (eapply exec_load_unchange_support; eauto)
+            | now (eapply exec_store_unchange_support; eauto)
+            | now (repeat destr_in H0)
+            | unfold goto_label in H0; repeat destr_in H0].
+  + rewrite (Mem.support_store _ _ _ _ _ _ Heqo1).
+    rewrite (Mem.support_store _ _ _ _ _ _ Heqo0).
+    eapply Mem.sup_include_trans. 2: eapply Mem.sup_include_record_frame; eauto.
+    apply Mem.sup_include_alloc in Heqp. simpl in Heqp.
+    eapply Mem.sup_include_trans. eapply Mem.sup_include_trans. 2:apply Heqp.
+    intro. eapply Mem.sup_incr_frame_in.
+    simpl. unfold Mem.sup_push_stage.  intro. destruct b; simpl; auto.
+  + erewrite <- Mem.support_free; eauto.
+    eapply Mem.sup_include_trans.
+    intro. eapply Mem.support_return_frame_1 in Heqo2. apply Heqo2.
+    eapply Mem.sup_include_pop_stage; eauto.
+Qed.
+
