x86/Asmgenproof.v
@@ -320,7 +320,7 @@ Lemma find_label_goto_label:
   rs PC = Vptr b ofs ->
   Mach.find_label lbl f.(Mach.fn_code) = Some c' ->
   exists tc', exists rs',
-    goto_label tf lbl rs m = Next rs' m
+    goto_label tge tf lbl rs m = Next rs' m
   /\ transl_code_at_pc ge (rs' PC) b f c' false tf tc'
   /\ forall r, r <> PC -> rs'#r = rs#r.
 Proof.
@@ -329,7 +329,8 @@ Proof.
   exploit label_pos_code_tail; eauto. instantiate (1 := 0).
   intros [pos' [P [Q R]]].
   exists tc; exists (rs#PC <- (Vptr b (Ptrofs.repr pos'))).
-  split. unfold goto_label. rewrite P. rewrite H1. auto.
+  split. unfold goto_label. rewrite P. exploit functions_transl; eauto.
+  intro. rewrite H1. rewrite H3. auto.
   split. rewrite Pregmap.gss. constructor; auto.
   rewrite Ptrofs.unsigned_repr. replace (pos' - 0) with pos' in Q.
   auto. lia.
@@ -435,7 +436,7 @@ Lemma exec_straight_steps_goto:
    exists jmp, exists k', exists rs2,
        exec_straight tge tf c rs1 m1' (jmp :: k') rs2 m2'
     /\ agree ms2 sp rs2
-    /\ exec_instr tge tf jmp rs2 m2' = goto_label tf lbl rs2 m2') ->
+    /\ exec_instr tge tf jmp rs2 m2' = goto_label tge tf lbl rs2 m2') ->
   exists st',
   plus step tge (State rs1 m1') E0 st' /\
   match_states (Mach.State s fb sp c' ms2 m2) st'.
