x86/SSAsmproof.v
@@ -1,0 +1,2135 @@
+Require Import Coqlib Errors.
+Require Import Integers Floats AST Linking.
+Require Import Values Memory Events Globalenvs Smallstep.
+Require Import Asm AsmFacts Asmgen Asmgenproof0.
+Require Import SSAsm.
+
+Section PRESERVATION.
+
+Variable prog: Asm.program.
+
+Let ge := Genv.globalenv prog.
+
+Definition stkblock := fresh_block (Genv.genv_sup ge).
+
+(** this hypothesis can be promised by asmgen *)
+Hypothesis prog_unchange_rsp: asm_prog_unchange_rsp ge.
+
+(** Memory Injection Lemmas *)
+Record meminj_preserves_globals (j: meminj) : Prop := { 
+  defs_inject: forall b gd,
+    Genv.find_def ge b = Some gd -> j b = Some (b, 0); 
+  defs_rev_inject: forall b b' delta gd,
+    j b = Some(b', delta) -> Genv.find_def ge b' = Some gd ->
+    b = b' /\ delta = 0;
+  symbol_inject: forall id b,
+    Genv.find_symbol ge id = Some b -> j b = Some(b, 0);  
+}.
+
+Lemma globals_symbols_inject:
+  forall j, meminj_preserves_globals j ->
+  symbols_inject j ge ge.
+Proof.
+  intros j GLOB_INJ.
+  repeat split; intros.
+  + simpl in H0. exploit symbol_inject; eauto. intro INJ. rewrite H in INJ. inv INJ. auto.
+  + simpl in H0. exploit symbol_inject; eauto. intro INJ. rewrite H in INJ. inv INJ. auto.
+  + simpl in H0. exploit symbol_inject; eauto. 
+  + simpl. unfold Genv.block_is_volatile.
+    destruct (Genv.find_var_info ge b1) as [gv|] eqn:V1.
+    rewrite Genv.find_var_info_iff in V1.
+    exploit defs_inject; eauto. intros A. rewrite H in A. inv A.
+    rewrite <- Genv.find_var_info_iff in V1. rewrite V1; auto.
+    destruct (Genv.find_var_info ge b2) as [gv|] eqn:V2; auto.
+    rewrite Genv.find_var_info_iff in V2.
+    exploit defs_rev_inject; eauto. intros (A & B). subst.
+    rewrite <- Genv.find_var_info_iff in V2. congruence.
+Qed.
+
+Lemma globinj_to_funinj:
+  forall (j: meminj),
+    meminj_preserves_globals j ->
+    forall b f, Genv.find_funct_ptr ge b = Some f -> j b = Some (b,0).
+Proof.
+  intros j MINJ b f FF. unfold Genv.find_funct_ptr in FF.  
+  exploit (defs_inject j MINJ b (Gfun f)); eauto.
+  repeat destr_in FF.
+Qed.
+
+(** Regset Injection Lemmas *)
+Lemma val_inject_set:
+  forall j rs1 rs2
+    (RINJ: forall r, Val.inject j (rs1 r) (rs2 r))
+    v v' (VINJ: Val.inject j v v') r1 r,
+    Val.inject j ((rs1 # r1 <- v) r) ((rs2 # r1 <- v') r).
+Proof.
+  intros.
+  destruct (PregEq.eq r1 r); subst; auto.
+  rewrite ! Pregmap.gss; auto.
+  rewrite ! Pregmap.gso by auto. auto.
+Qed.
+
+ Lemma val_inject_undef_regs:
+  forall l j rs1 rs2
+    (RINJ: forall r, Val.inject j (rs1 r) (rs2 r))
+    r,
+    Val.inject j (undef_regs l rs1 r) (undef_regs l rs2 r).
+Proof.
+  induction l; simpl; intros; eauto.
+  apply IHl.
+  intros; apply val_inject_set; auto.
+Qed.
+
+Lemma val_inject_undef_caller_save_regs:
+  forall j rs1 rs2
+    (RINJ: forall r, Val.inject j (rs1 r) (rs2 r))
+    r,
+    Val.inject j (undef_caller_save_regs rs1 r) (undef_caller_save_regs rs2 r).
+Proof.
+  intros; eauto.
+  unfold undef_caller_save_regs.
+  destruct (preg_eq r SP); destruct (in_dec preg_eq r (map preg_of (filter Conventions1.is_callee_save Machregs.all_mregs))); simpl; try (apply RINJ).
+  eauto.
+Qed.
+
+Lemma val_inject_nextinstr:
+  forall j rs1 rs2
+    (RINJ: forall r, Val.inject j (rs1 r) (rs2 r)) r,
+    Val.inject j (nextinstr rs1 r) (nextinstr rs2 r).
+Proof.
+  unfold nextinstr.
+  intros.
+  apply val_inject_set; auto.
+  apply Val.offset_ptr_inject; auto.
+Qed.
+
+Lemma val_inject_nextinstr_nf:
+  forall j rs1 rs2
+    (RINJ: forall r, Val.inject j (rs1 r) (rs2 r)) r,
+    Val.inject j (nextinstr_nf rs1 r) (nextinstr_nf rs2 r).
+Proof.
+  unfold nextinstr_nf.
+  intros.
+  apply val_inject_nextinstr; auto.
+  intros.
+  apply val_inject_undef_regs; auto.
+Qed.
+
+Lemma val_inject_set_res:
+  forall r rs1 rs2 v1 v2 j,
+    Val.inject j v1 v2 ->
+    (forall r0, Val.inject j (rs1 r0) (rs2 r0)) ->
+    forall r0, Val.inject j (set_res r v1 rs1 r0) (set_res r v2 rs2 r0).
+Proof.
+  induction r; simpl; intros; auto.
+  apply val_inject_set; auto.
+  eapply IHr2; eauto.
+  apply Val.loword_inject. auto.
+  intros; eapply IHr1; eauto.
+  apply Val.hiword_inject. auto.
+Qed.
+
+Lemma val_inject_set_pair:
+  forall j p res1 res2 rs1 rs2,
+    (forall r, Val.inject j (rs1 r) (rs2 r)) ->
+    Val.inject j res1 res2 ->
+    forall r,
+      Val.inject j (set_pair p res1 rs1 r) (set_pair p res2 rs2 r).
+Proof.
+  destruct p; simpl; intros; eauto.
+  apply val_inject_set; auto.
+  repeat (intros; apply val_inject_set; auto).
+  apply Val.hiword_inject; auto.
+  apply Val.loword_inject; auto.
+Qed.
+
+(** Stack Injection Lemmas *)
+Record single_stack_perm_ofs (m: mem) : Prop :=
+  {
+  stack_perm_offset: forall (ofs: Z) (k: perm_kind) (p: permission),
+      Mem.perm m stkblock ofs k p -> 0 <= ofs < Ptrofs.max_unsigned;
+  stack_offset_perm: forall (ofs: Z) (k: perm_kind) (p: permission),
+      0 <= ofs < Memory.max_stacksize -> Mem.perm m stkblock ofs k p;
+  }.
+
+Lemma stack_size_aligned :
+  forall stk,
+    (8 | Memory.stack_size stk).
+Proof.
+  intros. induction stk.
+  - simpl. apply Z.divide_0_r.
+  - induction a; simpl.
+    + auto.
+    + simpl in IHa.
+      generalize (Z.add_comm (Memory.size_of_all_frames a0) (Memory.stack_size stk)). intro. rewrite H in IHa.
+      exploit Z.divide_add_cancel_r. apply IHstk. apply IHa. intro.
+      assert (8 | align (Memory.frame_size a) 8). apply align_divides. lia.
+      repeat apply Z.divide_add_r; auto.
+Qed.
+
+(* Inductive inject_stack (j: meminj): Mem.stackadt -> Prop := *)
+(* | inject_stack_nil: *)
+(*     inject_stack j nil *)
+(* | inject_stack_cons_nil l (INJSTK_REC: inject_stack j l): *)
+(*     inject_stack j ((nil)::l) *)
+(* | inject_stack_cons *)
+(*     l fr b *)
+(*     (INJSTK_REC: inject_stack j l) *)
+(*     (INJBLOCK: j b = Some (stkblock, Mem.max_stacksize - Mem.stack_size l - Mem.frame_size fr)): *)
+(*     (BLOCKS: frame_block fr = b) *)
+(*     inject_stack j ((fr::nil)::l). *)
+
+(* Lemma inject_stack_incr: *)
+(*   forall j j' l *)
+(*     (INCR: inject_incr j j') *)
+(*     (IS: inject_stack j l), *)
+(*     inject_stack j' l. *)
+(* Proof. *)
+(*   induction 2; econstructor; eauto. *)
+(* Qed. *)
+
+Definition stack_inject_lowbound j m stklb:=
+  forall b delta ofs k p,
+    j b = Some (stkblock, delta) ->
+    Mem.perm m b ofs k p ->
+    stklb <= ofs + delta.
+
+(** matching state *)
+Inductive match_states: meminj -> state -> state -> Prop :=
+| match_states_intro:
+    forall (j: meminj)
+      (rs: regset) (m: mem) (rs': regset) (m': mem)
+   (** Memory Injection *)
+      (MINJ: Mem.inject j m m')
+      (GLOBINJ: meminj_preserves_globals j)
+      (ENVSUP: Mem.sup_include (Genv.genv_sup ge) (Mem.support m))
+      (ENVSUP': Mem.sup_include (Genv.genv_sup ge) (Mem.support m'))
+   (** Regset Injection *)
+      (RINJ: forall r, Val.inject j (rs # r) (rs' # r))
+   (** Stack Properties **)
+      (STKVB: Mem.valid_block m' stkblock)
+      (STKPERMOFS: single_stack_perm_ofs m')
+   (** Stack Injection *)
+      (RSPINJ: exists b, rs # RSP = Vptr b Ptrofs.zero)
+      (RSPINJ': exists stkofs,
+          (Ptrofs.unsigned stkofs =
+           Memory.max_stacksize -
+           Memory.stack_size (Mem.astack (Mem.support m)))
+          /\ rs' RSP = Vptr stkblock stkofs)
+      (STKINJLWBD: stack_inject_lowbound j m
+       (Memory.max_stacksize - Memory.stack_size (Mem.astack (Mem.support m)))),
+      match_states j (State rs m) (State rs' m').
+
+(** injection in exec_instr *)
+Section VAL_INJ_OPS.
+
+Variable f: meminj.
+
+Inductive opt_val_inject (j:meminj) : option val -> option val -> Prop :=
+| opt_val_inject_none v: opt_val_inject j None v
+| opt_val_inject_some v1 v2 : Val.inject j v1 v2 ->
+                              opt_val_inject j (Some v1) (Some v2).
+
+
+Remark zero_ext_inject:
+  forall v1 v2 n,
+    Val.inject f v1 v2 ->
+    Val.inject f (Val.zero_ext n v1) (Val.zero_ext n v2).
+Proof.
+  intros.
+  unfold Val.zero_ext. destruct v1, v2; auto; inv H; auto.
+Qed.
+
+Remark sign_ext_inject:
+  forall v1 v2 n,
+    Val.inject f v1 v2 ->
+    Val.inject f (Val.sign_ext n v1) (Val.sign_ext n v2).
+Proof.
+  intros.
+  unfold Val.sign_ext. destruct v1, v2; auto; inv H; auto.
+Qed.
+
+Remark longofintu_inject:
+  forall v1 v2,
+    Val.inject f v1 v2 ->
+    Val.inject f (Val.longofintu v1) (Val.longofintu v2).
+Proof.
+  intros.
+  unfold Val.longofintu. destruct v1, v2; auto; inv H; auto.
+Qed.
+
+Remark longofint_inject:
+  forall v1 v2,
+    Val.inject f v1 v2 ->
+    Val.inject f (Val.longofint v1) (Val.longofint v2).
+Proof.
+  intros.
+  unfold Val.longofint. destruct v1, v2; auto; inv H; auto.
+Qed.
+
+Remark singleoffloat_inject:
+  forall v1 v2,
+    Val.inject f v1 v2 ->
+    Val.inject f (Val.singleoffloat v1) (Val.singleoffloat v2).
+Proof.
+  intros.
+  unfold Val.singleoffloat. destruct v1, v2; auto; inv H; auto.
+Qed.
+ 
+Remark floatofsingle_inject:
+  forall v1 v2,
+    Val.inject f v1 v2 ->
+    Val.inject f (Val.floatofsingle v1) (Val.floatofsingle v2).
+Proof.
+  intros.
+  unfold Val.floatofsingle. destruct v1, v2; auto; inv H; auto.
+Qed.
+
+Remark maketotal_inject : forall v1 v2 j,
+    opt_val_inject j v1 v2 -> Val.inject j (Val.maketotal v1) (Val.maketotal v2).
+Proof.
+  intros.
+  inversion H; simpl; subst; auto.
+Qed.
+
+Remark intoffloat_inject : forall v1 v2,
+  Val.inject f v1 v2 -> opt_val_inject f (Val.intoffloat v1) (Val.intoffloat v2).
+Proof.
+  intros. unfold Val.intoffloat.
+  destruct v1; try (constructor); inv H.
+  destruct (Float.to_int f0); simpl; constructor; auto.
+Qed.
+
+Remark floatofint_inject : forall v1 v2,
+  Val.inject f v1 v2 -> opt_val_inject f (Val.floatofint v1) (Val.floatofint v2).
+Proof.
+  intros. unfold Val.floatofint.
+  destruct v1; try (constructor); inv H.
+  simpl; constructor; auto.
+Qed.
+
+Remark intofsingle_inject : forall v1 v2,
+  Val.inject f v1 v2 -> opt_val_inject f (Val.intofsingle v1) (Val.intofsingle v2).
+Proof.
+  intros. unfold Val.intofsingle.
+  destruct v1; try (constructor); inv H.
+  destruct (Float32.to_int f0); simpl; constructor; auto.
+Qed.
+
+Remark singleofint_inject : forall v1 v2,
+  Val.inject f v1 v2 -> opt_val_inject f (Val.singleofint v1) (Val.singleofint v2).
+Proof.
+  intros. unfold Val.singleofint.
+  destruct v1; try (constructor); inv H.
+  simpl; constructor; auto.
+Qed.
+
+Remark longoffloat_inject : forall v1 v2,
+  Val.inject f v1 v2 -> opt_val_inject f (Val.longoffloat v1) (Val.longoffloat v2).
+Proof.
+  intros. unfold Val.longoffloat.
+  destruct v1; try (constructor); inv H.
+  destruct (Float.to_long f0); simpl; constructor; auto.
+Qed.
+
+Remark floatoflong_inject : forall v1 v2,
+  Val.inject f v1 v2 -> opt_val_inject f (Val.floatoflong v1) (Val.floatoflong v2).
+Proof.
+  intros. unfold Val.floatoflong.
+  destruct v1; try (constructor); inv H.
+  simpl; constructor; auto.
+Qed.
+
+Remark longofsingle_inject : forall v1 v2,
+  Val.inject f v1 v2 -> opt_val_inject f (Val.longofsingle v1) (Val.longofsingle v2).
+Proof.
+  intros. unfold Val.longofsingle.
+  destruct v1; try (constructor); inv H.
+  destruct (Float32.to_long f0); simpl; constructor; auto.
+Qed.
+
+Remark singleoflong_inject : forall v1 v2,
+  Val.inject f v1 v2 -> opt_val_inject f (Val.singleoflong v1) (Val.singleoflong v2).
+Proof.
+  intros. unfold Val.singleoflong.
+  destruct v1; try (constructor); inv H.
+  simpl; constructor; auto.
+Qed.
+
+Remark neg_inject:
+  forall v1 v2,
+  Val.inject f v1 v2 ->
+  Val.inject f (Val.neg v1) (Val.neg v2).
+Proof.
+  intros.
+  unfold Val.neg. destruct v1, v2; auto; inv H; auto.
+Qed.
+
+Remark negl_inject:
+  forall v1 v2,
+  Val.inject f v1 v2 ->
+  Val.inject f (Val.negl v1) (Val.negl v2).
+Proof.
+  intros.
+  unfold Val.negl. destruct v1, v2; auto; inv H; auto.
+Qed.
+
+Remark mul_inject:
+  forall v1 v1' v2 v2',
+  Val.inject f v1 v1' ->
+  Val.inject f v2 v2' ->
+  Val.inject f (Val.mul v1 v2) (Val.mul v1' v2').
+Proof.
+  intros.
+  unfold Val.mul. destruct v1, v2; auto; inv H; inv H0; auto.
+Qed.
+
+Remark mull_inject:
+  forall v1 v1' v2 v2',
+  Val.inject f v1 v1' ->
+  Val.inject f v2 v2' ->
+  Val.inject f (Val.mull v1 v2) (Val.mull v1' v2').
+Proof.
+  intros.
+  unfold Val.mull. destruct v1, v2; auto; inv H; inv H0; auto.
+Qed.
+
+Remark mulhs_inject:
+  forall v1 v1' v2 v2',
+  Val.inject f v1 v1' ->
+  Val.inject f v2 v2' ->
+  Val.inject f (Val.mulhs v1 v2) (Val.mulhs v1' v2').
+Proof.
+  intros.
+  unfold Val.mulhs. destruct v1, v2; auto; inv H; inv H0; auto.
+Qed.
+
+Remark mullhs_inject:
+  forall v1 v1' v2 v2',
+  Val.inject f v1 v1' ->
+  Val.inject f v2 v2' ->
+  Val.inject f (Val.mullhs v1 v2) (Val.mullhs v1' v2').
+Proof.
+  intros.
+  unfold Val.mullhs. destruct v1, v2; auto; inv H; inv H0; auto.
+Qed.
+
+Remark mulhu_inject:
+  forall v1 v1' v2 v2',
+  Val.inject f v1 v1' ->
+  Val.inject f v2 v2' ->
+  Val.inject f (Val.mulhu v1 v2) (Val.mulhu v1' v2').
+Proof.
+  intros.
+  unfold Val.mulhu. destruct v1, v2; auto; inv H; inv H0; auto.
+Qed.
+
+Remark mullhu_inject:
+  forall v1 v1' v2 v2',
+  Val.inject f v1 v1' ->
+  Val.inject f v2 v2' ->
+  Val.inject f (Val.mullhu v1 v2) (Val.mullhu v1' v2').
+Proof.
+  intros.
+  unfold Val.mullhu. destruct v1, v2; auto; inv H; inv H0; auto.
+Qed.
+
+Remark shr_inject:
+  forall v1 v1' v2 v2',
+  Val.inject f v1 v1' ->
+  Val.inject f v2 v2' ->
+  Val.inject f (Val.shr v1 v2) (Val.shr v1' v2').
+Proof.
+  intros.
+  unfold Val.shr. destruct v1, v2; auto; inv H; inv H0.
+  destruct (Int.ltu i0 Int.iwordsize); auto.
+Qed.
+
+Remark shrl_inject:
+  forall v1 v1' v2 v2',
+  Val.inject f v1 v1' ->
+  Val.inject f v2 v2' ->
+  Val.inject f (Val.shrl v1 v2) (Val.shrl v1' v2').
+Proof.
+  intros.
+  unfold Val.shrl. destruct v1, v2; auto; inv H; inv H0.
+  destruct (Int.ltu i0 Int64.iwordsize'); auto.
+Qed.
+
+Remark and_inject:
+  forall v1 v1' v2 v2',
+  Val.inject f v1 v1' ->
+  Val.inject f v2 v2' ->
+  Val.inject f (Val.and v1 v2) (Val.and v1' v2').
+Proof.
+  intros.
+  unfold Val.and. destruct v1, v2; auto; inv H; inv H0.
+  auto.
+Qed.
+
+Remark andl_inject:
+  forall v1 v1' v2 v2',
+  Val.inject f v1 v1' ->
+  Val.inject f v2 v2' ->
+  Val.inject f (Val.andl v1 v2) (Val.andl v1' v2').
+Proof.
+  intros.
+  unfold Val.andl. destruct v1, v2; auto; inv H; inv H0.
+  auto.
+Qed.
+
+Remark or_inject:
+  forall v1 v1' v2 v2',
+  Val.inject f v1 v1' ->
+  Val.inject f v2 v2' ->
+  Val.inject f (Val.or v1 v2) (Val.or v1' v2').
+Proof.
+  intros.
+  unfold Val.or. destruct v1, v2; auto; inv H; inv H0.
+  auto.
+Qed.
+
+Remark orl_inject:
+  forall v1 v1' v2 v2',
+  Val.inject f v1 v1' ->
+  Val.inject f v2 v2' ->
+  Val.inject f (Val.orl v1 v2) (Val.orl v1' v2').
+Proof.
+  intros.
+  unfold Val.orl. destruct v1, v2; auto; inv H; inv H0.
+  auto.
+Qed.
+
+Remark xor_inject:
+  forall v1 v1' v2 v2',
+  Val.inject f v1 v1' ->
+  Val.inject f v2 v2' ->
+  Val.inject f (Val.xor v1 v2) (Val.xor v1' v2').
+Proof.
+  intros.
+  unfold Val.xor. destruct v1, v2; auto; inv H; inv H0.
+  auto.
+Qed.
+
+Remark xorl_inject:
+  forall v1 v1' v2 v2',
+  Val.inject f v1 v1' ->
+  Val.inject f v2 v2' ->
+  Val.inject f (Val.xorl v1 v2) (Val.xorl v1' v2').
+Proof.
+  intros.
+  unfold Val.xorl. destruct v1, v2; auto; inv H; inv H0.
+  auto.
+Qed.
+
+Remark notint_inject:
+  forall v1 v2,
+  Val.inject f v1 v2 ->
+  Val.inject f (Val.notint v1) (Val.notint v2).
+Proof.
+  intros.
+  unfold Val.notint. destruct v1, v2; auto; inv H; auto.
+Qed.
+
+Remark notl_inject:
+  forall v1 v2,
+  Val.inject f v1 v2 ->
+  Val.inject f (Val.notl v1) (Val.notl v2).
+Proof.
+  intros.
+  unfold Val.notl. destruct v1, v2; auto; inv H; auto.
+Qed.
+
+Remark shl_inject:
+  forall v1 v1' v2 v2',
+  Val.inject f v1 v1' ->
+  Val.inject f v2 v2' ->
+  Val.inject f (Val.shl v1 v2) (Val.shl v1' v2').
+Proof.
+  intros.
+  unfold Val.shl. destruct v1, v2; auto; inv H; inv H0.
+  destruct (Int.ltu i0 Int.iwordsize); auto.
+Qed.
+
+Remark shll_inject:
+  forall v1 v1' v2 v2',
+  Val.inject f v1 v1' ->
+  Val.inject f v2 v2' ->
+  Val.inject f (Val.shll v1 v2) (Val.shll v1' v2').
+Proof.
+  intros.
+  unfold Val.shll. destruct v1, v2; auto; inv H; inv H0.
+  destruct (Int.ltu i0 Int64.iwordsize'); auto.
+Qed.
+
+Remark shru_inject:
+  forall v1 v1' v2 v2',
+  Val.inject f v1 v1' ->
+  Val.inject f v2 v2' ->
+  Val.inject f (Val.shru v1 v2) (Val.shru v1' v2').
+Proof.
+  intros.
+  unfold Val.shru. destruct v1, v2; auto; inv H; inv H0.
+  destruct (Int.ltu i0 Int.iwordsize); auto.
+Qed.
+
+Remark shrlu_inject:
+  forall v1 v1' v2 v2',
+  Val.inject f v1 v1' ->
+  Val.inject f v2 v2' ->
+  Val.inject f (Val.shrlu v1 v2) (Val.shrlu v1' v2').
+Proof.
+  intros.
+  unfold Val.shrlu. destruct v1, v2; auto; inv H; inv H0.
+  destruct (Int.ltu i0 Int64.iwordsize'); auto.
+Qed.
+
+Remark ror_inject:
+  forall v1 v1' v2 v2',
+  Val.inject f v1 v1' ->
+  Val.inject f v2 v2' ->
+  Val.inject f (Val.ror v1 v2) (Val.ror v1' v2').
+Proof.
+  intros.
+  unfold Val.ror. destruct v1, v2; auto; inv H; inv H0.
+  destruct (Int.ltu i0 Int.iwordsize); auto.
+Qed.
+
+Remark rorl_inject:
+  forall v1 v1' v2 v2',
+  Val.inject f v1 v1' ->
+  Val.inject f v2 v2' ->
+  Val.inject f (Val.rorl v1 v2) (Val.rorl v1' v2').
+Proof.
+  intros.
+  unfold Val.rorl. destruct v1, v2; auto; inv H; inv H0.
+  destruct (Int.ltu i0 Int64.iwordsize'); auto.
+Qed.
+
+Lemma weak_valid_pointer_nonempty_perm:
+  forall m b ofs,
+  Mem.weak_valid_pointer m b ofs = true <-> 
+  (Mem.perm m b ofs Cur Nonempty) \/ (Mem.perm m b (ofs-1) Cur Nonempty).
+Proof.
+  intros. unfold Mem.weak_valid_pointer. unfold Mem.valid_pointer.
+  destruct (Mem.perm_dec m b ofs Cur Nonempty); destruct (Mem.perm_dec m b (ofs-1) Cur Nonempty); simpl;
+  intuition congruence.
+Qed.
+
+Lemma weak_valid_pointer_size_bounds : forall f b1 b2 m1 m2 ofs delta,
+  f b1 = Some (b2, delta) ->
+  Mem.inject f m1 m2 ->
+  Mem.weak_valid_pointer m1 b1 (Ptrofs.unsigned ofs) = true ->
+  0 <= delta <= Ptrofs.max_unsigned /\
+  0 <= Ptrofs.unsigned ofs + delta <= Ptrofs.max_unsigned.
+Proof.
+  intros. exploit Mem.mi_representable; eauto.
+  rewrite weak_valid_pointer_nonempty_perm in H1.
+  destruct H1; eauto with mem. intros.
+  generalize (Ptrofs.unsigned_range ofs). lia.
+Qed.
+
+Theorem valid_pointer_inject_ofs:
+  forall f m1 m2 b1 ofs b2 delta,
+  f b1 = Some(b2, delta) ->
+  Mem.inject f m1 m2 ->
+  Mem.valid_pointer m1 b1 (Ptrofs.unsigned ofs) = true ->
+  Mem.valid_pointer m2 b2  (Ptrofs.unsigned (Ptrofs.add ofs (Ptrofs.repr delta))) = true.
+Proof.
+  intros. exploit Mem.valid_pointer_inject; eauto. intros.
+  intros. unfold Ptrofs.add.
+  exploit weak_valid_pointer_size_bounds; eauto.
+  erewrite Mem.weak_valid_pointer_spec; eauto.
+  intros [A B].
+  repeat rewrite Ptrofs.unsigned_repr; eauto.
+Qed.
+
+Theorem weak_valid_pointer_inject_ofs: 
+  forall f m1 m2 b1 ofs b2 delta,
+  f b1 = Some(b2, delta) ->
+  Mem.inject f m1 m2 ->
+  Mem.weak_valid_pointer m1 b1 (Ptrofs.unsigned ofs) = true ->
+  Mem.weak_valid_pointer m2 b2 (Ptrofs.unsigned (Ptrofs.add ofs (Ptrofs.repr delta))) = true.
+Proof.
+  intros. exploit Mem.weak_valid_pointer_inject; eauto.
+  intros. unfold Ptrofs.add.
+  exploit weak_valid_pointer_size_bounds; eauto. intros [A B].
+  repeat rewrite Ptrofs.unsigned_repr; auto.
+Qed.
+
+Remark vtrue_inject : 
+  Val.inject f Vtrue Vtrue.
+Proof.
+  intros. unfold Vtrue. auto.
+Qed.
+
+Remark vfalse_inject : 
+  Val.inject f Vfalse Vfalse.
+Proof.
+  intros. unfold Vfalse. auto.
+Qed.
+
+Remark vofbool_inject : forall v,
+  Val.inject f (Val.of_bool v) (Val.of_bool v).
+Proof.
+  destruct v; simpl.
+  - apply vtrue_inject.
+  - apply vfalse_inject.
+Qed.
+
+Definition cmpu_bool_inject := fun j m m' (MINJ: Mem.inject j m m') => Val.cmpu_bool_inject j (Mem.valid_pointer m) (Mem.valid_pointer m') (fun b1 ofs b2 delta FB => valid_pointer_inject_ofs j m m' b1 ofs b2 delta FB MINJ) (fun b1 ofs b2 delta FB => weak_valid_pointer_inject_ofs j m m' b1 ofs b2 delta FB MINJ) (fun b ofs b' delta FB MVP => Mem.weak_valid_pointer_inject_no_overflow j m m' b ofs b' delta MINJ MVP FB) (fun b1 ofs1 b2 ofs2 b1' delta1 b2' delta2 => Mem.different_pointers_inject j m m' b1  ofs1 b2 ofs2 b1' delta1 b2' delta2 MINJ).
+
+Remark cmpu_inject
+  : forall (m m' : mem),
+    Mem.inject f m m' ->
+    forall (c : comparison) (v1 v2 v1' v2' : val),
+      Val.inject f v1 v1' ->
+      Val.inject f v2 v2' ->
+      Val.inject f (Val.cmpu (Mem.valid_pointer m) c v1 v2)
+                 (Val.cmpu (Mem.valid_pointer m') c v1' v2').
+Proof.
+  unfold Val.cmpu. unfold Val.of_optbool.
+  intros.
+  destr. eapply cmpu_bool_inject in Heqo; eauto.
+  rewrite Heqo. unfold Vtrue, Vfalse; destr; auto. auto.
+Qed.
+
+Definition cmplu_bool_inject := fun j m m' (MINJ: Mem.inject j m m') => Val.cmplu_bool_inject j (Mem.valid_pointer m) (Mem.valid_pointer m') (fun b1 ofs b2 delta FB => valid_pointer_inject_ofs j m m' b1 ofs b2 delta FB MINJ) (fun b1 ofs b2 delta FB => weak_valid_pointer_inject_ofs j m m' b1 ofs b2 delta FB MINJ) (fun b ofs b' delta FB MVP => Mem.weak_valid_pointer_inject_no_overflow j m m' b ofs b' delta MINJ MVP FB) (fun b1 ofs1 b2 ofs2 b1' delta1 b2' delta2 => Mem.different_pointers_inject j m m' b1  ofs1 b2 ofs2 b1' delta1 b2' delta2 MINJ).
+
+Remark cmplu_inject
+  : forall (m m' : mem),
+    Mem.inject f m m' ->
+    forall (c : comparison) (v1 v2 v1' v2' : val),
+      Val.inject f v1 v1' ->
+      Val.inject f v2 v2' ->
+      opt_val_inject f (Val.cmplu (Mem.valid_pointer m) c v1 v2)
+                     (Val.cmplu (Mem.valid_pointer m') c v1' v2').
+Proof.
+  unfold Val.cmplu. unfold option_map.
+  intros.
+  destr. eapply cmplu_bool_inject in Heqo; eauto.
+  rewrite Heqo. constructor. apply vofbool_inject. constructor.
+Qed.
+
+Remark negative_inject:
+  forall v v',
+    Val.inject f v v' ->
+    Val.inject f (Val.negative v) (Val.negative v').
+Proof.
+  unfold Val.negative. intros.
+  destr; auto. inv H. auto.
+Qed.
+
+Remark negativel_inject:
+  forall v v',
+    Val.inject f v v' ->
+    Val.inject f (Val.negativel v) (Val.negativel v').
+Proof.
+  unfold Val.negativel. intros.
+  destr; auto. inv H. auto.
+Qed.
+
+Remark sub_overflow_inject:
+  forall v1 v2 v3 v4,
+    Val.inject f v1 v2 ->
+    Val.inject f v3 v4 ->
+    Val.inject f (Val.sub_overflow v1 v3) (Val.sub_overflow v2 v4).
+Proof.
+  unfold Val.sub_overflow; intros.
+  destr; auto. inv H. destr; auto; inv H0. auto.
+Qed.
+
+Remark subl_overflow_inject:
+  forall v1 v2 v3 v4,
+    Val.inject f v1 v2 ->
+    Val.inject f v3 v4 ->
+    Val.inject f (Val.subl_overflow v1 v3) (Val.subl_overflow v2 v4).
+Proof.
+  unfold Val.subl_overflow; intros.
+  destr; auto. inv H. destr; auto; inv H0. auto.
+Qed.
+
+Remark addf_inject:
+  forall v1 v1' v2 v2',
+  Val.inject f v1 v1' ->
+  Val.inject f v2 v2' ->
+  Val.inject f (Val.addf v1 v2) (Val.addf v1' v2').
+Proof.
+  intros.
+  unfold Val.addf. destruct v1, v2; auto; inv H; inv H0.
+  auto.
+Qed.
+
+Remark subf_inject:
+  forall v1 v1' v2 v2',
+  Val.inject f v1 v1' ->
+  Val.inject f v2 v2' ->
+  Val.inject f (Val.subf v1 v2) (Val.subf v1' v2').
+Proof.
+  intros.
+  unfold Val.subf. destruct v1, v2; auto; inv H; inv H0.
+  auto.
+Qed.
+
+Remark mulf_inject:
+  forall v1 v1' v2 v2',
+  Val.inject f v1 v1' ->
+  Val.inject f v2 v2' ->
+  Val.inject f (Val.mulf v1 v2) (Val.mulf v1' v2').
+Proof.
+  intros.
+  unfold Val.mulf. destruct v1, v2; auto; inv H; inv H0.
+  auto.
+Qed.
+
+Remark divf_inject:
+  forall v1 v1' v2 v2',
+  Val.inject f v1 v1' ->
+  Val.inject f v2 v2' ->
+  Val.inject f (Val.divf v1 v2) (Val.divf v1' v2').
+Proof.
+  intros.
+  unfold Val.divf. destruct v1, v2; auto; inv H; inv H0.
+  auto.
+Qed.
+
+Remark negf_inject:
+  forall v v',
+    Val.inject f v v' ->
+    Val.inject f (Val.negf v) (Val.negf v').
+Proof.
+  intros.
+  unfold Val.negf. destr; auto. inv H. auto.
+Qed.
+
+Remark absf_inject:
+  forall v v',
+    Val.inject f v v' ->
+    Val.inject f (Val.absf v) (Val.absf v').
+Proof.
+  intros.
+  unfold Val.absf. destr; auto. inv H. auto.
+Qed.
+
+Remark addfs_inject:
+  forall v1 v1' v2 v2',
+  Val.inject f v1 v1' ->
+  Val.inject f v2 v2' ->
+  Val.inject f (Val.addfs v1 v2) (Val.addfs v1' v2').
+Proof.
+  intros.
+  unfold Val.addfs. destruct v1, v2; auto; inv H; inv H0.
+  auto.
+Qed.
+
+Remark subfs_inject:
+  forall v1 v1' v2 v2',
+  Val.inject f v1 v1' ->
+  Val.inject f v2 v2' ->
+  Val.inject f (Val.subfs v1 v2) (Val.subfs v1' v2').
+Proof.
+  intros.
+  unfold Val.subfs. destruct v1, v2; auto; inv H; inv H0.
+  auto.
+Qed.
+
+Remark mulfs_inject:
+  forall v1 v1' v2 v2',
+  Val.inject f v1 v1' ->
+  Val.inject f v2 v2' ->
+  Val.inject f (Val.mulfs v1 v2) (Val.mulfs v1' v2').
+Proof.
+  intros.
+  unfold Val.mulfs. destruct v1, v2; auto; inv H; inv H0.
+  auto.
+Qed.
+
+Remark divfs_inject:
+  forall v1 v1' v2 v2',
+  Val.inject f v1 v1' ->
+  Val.inject f v2 v2' ->
+  Val.inject f (Val.divfs v1 v2) (Val.divfs v1' v2').
+Proof.
+  intros.
+  unfold Val.divfs. destruct v1, v2; auto; inv H; inv H0.
+  auto.
+Qed.
+
+Remark negfs_inject:
+  forall v v',
+    Val.inject f v v' ->
+    Val.inject f (Val.negfs v) (Val.negfs v').
+Proof.
+  intros.
+  unfold Val.negfs. destr; auto. inv H. auto.
+Qed.
+
+Remark absfs_inject:
+  forall v v',
+    Val.inject f v v' ->
+    Val.inject f (Val.absfs v) (Val.absfs v').
+Proof.
+  intros.
+  unfold Val.absfs. destr; auto. inv H. auto.
+Qed.
+
+End VAL_INJ_OPS.
+
+Lemma symbol_address_inject:
+  forall j id ofs,
+    meminj_preserves_globals j ->
+    Val.inject j (Genv.symbol_address ge id ofs) (Genv.symbol_address ge id ofs).
+Proof.
+  intros j id i0 MPG.
+  destruct MPG. unfold Genv.symbol_address. simpl in symbol_inject0. destr; auto. apply symbol_inject0 in Heqo.
+  econstructor; eauto.
+  rewrite Ptrofs.add_zero. auto.
+Qed.
+
+Lemma eval_addrmode32_inject:
+  forall a rs rs' j,
+    meminj_preserves_globals j ->
+    (forall r, Val.inject j (rs r) (rs' r)) ->
+    Val.inject j (eval_addrmode32 ge a rs) (eval_addrmode32 ge a rs').
+Proof.
+  unfold eval_addrmode32. intros.
+  destruct a.
+  apply Val.add_inject. destr; auto.
+  apply Val.add_inject. repeat destr; eauto using mul_inject.
+  repeat destr; eauto using symbol_address_inject.
+Qed.
+
+Lemma eval_addrmode64_inject:
+  forall a rs rs' j,
+    meminj_preserves_globals j ->
+    (forall r, Val.inject j (rs r) (rs' r)) ->
+    Val.inject j (eval_addrmode64 ge a rs) (eval_addrmode64 ge a rs').
+Proof.
+  unfold eval_addrmode64. intros.
+  destruct a.
+  apply Val.addl_inject. destr; auto.
+  apply Val.addl_inject. repeat destr; eauto using mull_inject.
+  repeat destr; eauto using symbol_address_inject.
+Qed.
+
+Lemma eval_addrmode_inject:
+  forall a rs rs' j,
+    meminj_preserves_globals j ->
+    (forall r, Val.inject j (rs r) (rs' r)) ->
+    Val.inject j (eval_addrmode ge a rs) (eval_addrmode ge a rs').
+Proof.
+  unfold eval_addrmode.
+  intros.
+  destr; eauto using eval_addrmode32_inject, eval_addrmode64_inject.
+Qed.
+
+Lemma exec_load_inject:
+  forall κ m1 a rs1 rd rs1' m1' rs2 m2 j,
+    meminj_preserves_globals j ->
+    Mem.inject j m1 m2 ->
+    (forall r, Val.inject j (rs1 r) (rs2 r)) ->
+    exec_load ge κ m1 a rs1 rd = Next rs1' m1' ->
+    exists rs2' m2',
+      exec_load ge κ m2 a rs2 rd = Next rs2' m2' /\
+      Mem.inject j m1' m2' /\
+      forall r, Val.inject j (rs1' r) (rs2' r).
+Proof.
+  unfold exec_load.
+  intros κ m1 a rs1 rd rs1' m1' rs2 m2 j MPG MINJ RINJ EL.
+  destr_in EL. inv EL.
+  edestruct Mem.loadv_inject as (v2 & LD & VINJ); eauto.
+  apply eval_addrmode_inject; auto.
+  rewrite LD. do 2 eexists; split; eauto. split; auto.
+  intros; apply val_inject_nextinstr_nf.
+  intros; apply val_inject_set; auto.
+Qed.
+
+Lemma exec_store_inject:
+  forall κ m1 a rs1 rd rs1' m1' rs2 m2 j destroyed,
+    meminj_preserves_globals j ->
+    Mem.inject j m1 m2 ->
+    (forall r, Val.inject j (rs1 r) (rs2 r)) ->
+    exec_store ge κ m1 a rs1 rd destroyed = Next rs1' m1' ->
+    exists rs2' m2',
+      exec_store ge κ m2 a rs2 rd destroyed = Next rs2' m2' /\
+      Mem.inject j m1' m2' /\
+      forall r, Val.inject j (rs1' r) (rs2' r).
+Proof.
+  unfold exec_store. intros κ m1 a rs1 rd rs1' m1' rs2 m2 j destroyed MPG MINJ RINJ ES.
+  destr_in ES. inv ES.
+  edestruct Mem.storev_mapped_inject as (m2' & ST & MINJ'); eauto.
+  apply eval_addrmode_inject; auto.
+  rewrite ST. do 2 eexists; split; eauto. split; auto.
+  intros; apply val_inject_nextinstr_nf.
+  intros; apply val_inject_undef_regs; auto.
+Qed.
+
+
+Ltac simpl_inject :=
+  first [
+      apply val_inject_nextinstr
+    | apply val_inject_nextinstr_nf
+    | apply val_inject_set
+    | apply val_inject_undef_regs
+    | apply Val.offset_ptr_inject
+    | apply Val.loword_inject
+    | apply Val.hiword_inject
+    | apply Val.add_inject
+    | apply Val.sub_inject
+    | apply Val.addl_inject
+    | apply Val.subl_inject
+    | apply eval_addrmode32_inject
+    | apply eval_addrmode64_inject
+    | apply eval_addrmode_inject
+    | apply symbol_address_inject
+    | apply zero_ext_inject
+    | apply sign_ext_inject
+    | apply longofintu_inject
+    | apply longofint_inject
+    | apply singleoffloat_inject
+    | apply floatofsingle_inject
+    | apply maketotal_inject
+    | apply intoffloat_inject
+    | apply floatofint_inject
+    | apply intofsingle_inject
+    | apply singleofint_inject
+    | apply longoffloat_inject
+    | apply floatoflong_inject
+    | apply longofsingle_inject
+    | apply singleoflong_inject
+    | apply neg_inject
+    | apply negl_inject
+    | apply mul_inject
+    | apply mull_inject
+    | apply mulhs_inject
+    | apply mullhs_inject
+    | apply mulhu_inject
+    | apply mullhu_inject
+    | apply shr_inject
+    | apply shrl_inject
+    | apply and_inject
+    | apply andl_inject
+    | apply or_inject
+    | apply orl_inject
+    | apply xor_inject
+    | apply xorl_inject
+    | apply notint_inject
+    | apply notl_inject
+    | apply shl_inject
+    | apply shll_inject
+    | apply shru_inject
+    | apply shrlu_inject
+    | apply ror_inject
+    | apply rorl_inject
+    | apply cmpu_inject
+    | apply cmplu_inject
+    | apply negative_inject
+    | apply negativel_inject
+    | apply sub_overflow_inject
+    | apply subl_overflow_inject
+    | apply addf_inject
+    | apply subf_inject
+    | apply mulf_inject
+    | apply divf_inject
+    | apply negf_inject
+    | apply absf_inject
+    | apply addfs_inject
+    | apply subfs_inject
+    | apply mulfs_inject
+    | apply divfs_inject
+    | apply negfs_inject
+    | apply absfs_inject
+    | unfold Vzero; auto
+    ].
+
+Lemma eval_testcond_inject:
+  forall j rs1 rs2
+    (RINJ : forall r : PregEq.t, Val.inject j (rs1 r) (rs2 r)) c b,
+    eval_testcond c rs1 = Some b ->
+    eval_testcond c rs2 = Some b.
+Proof.
+  unfold eval_testcond.
+  intros.
+  generalize (RINJ ZF), (RINJ CF), (RINJ OF), (RINJ SF), (RINJ PF).
+  intros A B C D E.
+  repeat destr_in H;
+    repeat match goal with
+           | H: Val.inject _ (Vint _) _ |- _ => inv H
+           | |- _ => simpl; auto
+           end.
+Qed.
+
+Lemma eval_testcond_of_optbool_inject:
+  forall j rs1 rs2
+    (RINJ : forall r : PregEq.t, Val.inject j (rs1 r) (rs2 r)) c,
+    Val.inject j (Val.of_optbool (eval_testcond c rs1)) (Val.of_optbool (eval_testcond c rs2)).
+Proof.
+  unfold Val.of_optbool. intros.
+  destr. erewrite eval_testcond_inject; eauto.
+  unfold Vtrue, Vfalse; destr; eauto. auto.
+Qed.
+
+Lemma compare_floats_inject:
+  forall j rs1 rs2
+    (RINJ : forall r : PregEq.t, Val.inject j (rs1 r) (rs2 r)) a b c d
+    (INJ1: Val.inject j a c) (INJ2: Val.inject j b d) r,
+    Val.inject j (compare_floats a b rs1 r) (compare_floats c d rs2 r).
+Proof.
+  unfold compare_floats.
+  intros.
+  inv INJ1; repeat simpl_inject.
+  inv INJ2; repeat simpl_inject.
+  apply vofbool_inject.
+  apply vofbool_inject.
+  apply vofbool_inject.
+  repeat (destr; repeat simpl_inject).
+  repeat (destr; repeat simpl_inject).
+Qed.
+
+Lemma compare_floats32_inject:
+  forall j rs1 rs2
+    (RINJ : forall r : PregEq.t, Val.inject j (rs1 r) (rs2 r)) a b c d
+    (INJ1: Val.inject j a c) (INJ2: Val.inject j b d) r,
+    Val.inject j (compare_floats32 a b rs1 r) (compare_floats32 c d rs2 r).
+Proof.
+  unfold compare_floats32.
+  intros.
+  inv INJ1; repeat simpl_inject.
+  inv INJ2; repeat simpl_inject.
+  apply vofbool_inject.
+  apply vofbool_inject.
+  apply vofbool_inject.
+  repeat (destr; repeat simpl_inject).
+  repeat (destr; repeat simpl_inject).
+Qed.
+
+Lemma goto_label_inject:
+  forall j rs1 rs2 m1 m2
+    (MINJ: Mem.inject j m1 m2)
+    (GLOBFUN_INJ: forall b f, Genv.find_funct_ptr ge b = Some f -> j b = Some (b,0))
+    (RINJ : forall r : PregEq.t, Val.inject j (rs1 r) (rs2 r))
+    l f rs1' m1',
+    Asm.goto_label ge f l rs1 m1 = Next rs1' m1' ->
+    exists rs2' m2',
+      Asm.goto_label ge f l rs2 m2 = Next rs2' m2' /\
+      Mem.inject j m1' m2' /\
+      forall r, Val.inject j (rs1' r) (rs2' r).
+Proof.
+  unfold goto_label. intros. repeat destr_in H.
+  generalize (RINJ PC); rewrite Heqv. intro A; inv A.
+  erewrite GLOBFUN_INJ in H2; eauto. inv H2. rewrite Heqo0.
+  do 2 eexists; split; eauto. split; eauto.
+  repeat simpl_inject. econstructor; eauto. rewrite Ptrofs.add_zero. auto.
+Qed.
+
+Lemma exec_instr_inject_normal:
+  forall j m1 m2 rs1 rs2 f i rs1' m1'
+    (MINJ: Mem.inject j m1 m2)
+    (GLOBINJ: meminj_preserves_globals j)
+    (RINJ: forall r, Val.inject j (rs1 # r) (rs2 # r))
+    (NOTSTKINSTR: stk_unrelated_instr i = true)
+    (EI: Asm.exec_instr ge f i rs1 m1 = Next rs1' m1'),
+  exists rs2' m2',
+    Asm.exec_instr ge f i rs2 m2 = Next rs2' m2'
+    /\ Mem.inject j m1' m2'
+    /\ (forall r, Val.inject j (rs1' # r) (rs2' # r)).
+Proof.
+  intros.
+  destruct i; (simpl in *; repeat destr_in EI;
+               try congruence;
+
+               match goal with
+               | |- exists _ _, Next _ _ = Next _ _ /\ _ /\ _ =>
+                 try (do 2 eexists; split; [now eauto |
+                                            split; [
+                                              eauto with mem
+                                            | repeat
+                                                simpl_inject
+                                            ]
+                                           ]
+                     )
+               | |- _ => try first [
+                             now (eapply exec_load_inject; eauto)
+                           | now (eapply exec_store_inject; eauto)
+                           ]
+               end
+              ).
+  + generalize (RINJ RDX); rewrite Heqv; inversion 1; subst.
+    generalize (RINJ RAX); rewrite Heqv0; inversion 1; subst.
+    generalize (RINJ r1); rewrite Heqv1; inversion 1; subst.
+    rewrite Heqo.
+    do 2 eexists; split; eauto. split; eauto. repeat simpl_inject.
+  + generalize (RINJ RDX); rewrite Heqv; inversion 1; subst.
+    generalize (RINJ RAX); rewrite Heqv0; inversion 1; subst.
+    generalize (RINJ r1); rewrite Heqv1; inversion 1; subst.
+    rewrite Heqo.
+    do 2 eexists; split; eauto. split; eauto. repeat simpl_inject.
+  + generalize (RINJ RDX); rewrite Heqv; inversion 1; subst.
+    generalize (RINJ RAX); rewrite Heqv0; inversion 1; subst.
+    generalize (RINJ r1); rewrite Heqv1; inversion 1; subst.
+    rewrite Heqo.
+    do 2 eexists; split; eauto. split; eauto. repeat simpl_inject.
+  + generalize (RINJ RDX); rewrite Heqv; inversion 1; subst.
+    generalize (RINJ RAX); rewrite Heqv0; inversion 1; subst.
+    generalize (RINJ r1); rewrite Heqv1; inversion 1; subst.
+    rewrite Heqo.
+    do 2 eexists; split; eauto. split; eauto. repeat simpl_inject.
+  + erewrite eval_testcond_inject; eauto. simpl. auto.
+  + erewrite eval_testcond_inject; eauto. simpl. auto.
+  + eapply eval_testcond_of_optbool_inject. auto.
+  + eapply compare_floats_inject; auto.
+  + eapply compare_floats32_inject; auto.
+  + eapply goto_label_inject; eauto.
+    eapply globinj_to_funinj. auto.
+  + erewrite eval_testcond_inject; eauto. simpl.
+    eapply goto_label_inject; eauto. eapply globinj_to_funinj. auto.
+  + erewrite eval_testcond_inject; eauto. simpl.
+    do 2 eexists; split; eauto. split; eauto. repeat simpl_inject.
+  + erewrite eval_testcond_inject; eauto. simpl.
+    erewrite eval_testcond_inject; eauto. simpl.
+    eapply goto_label_inject; eauto. eapply globinj_to_funinj. auto.
+  + erewrite eval_testcond_inject; eauto. simpl.
+    erewrite eval_testcond_inject; eauto. simpl.
+    do 2 eexists; split; eauto. split; eauto. repeat simpl_inject.
+  + erewrite eval_testcond_inject; eauto. simpl.
+    erewrite eval_testcond_inject; eauto. simpl.
+    do 2 eexists; split; eauto. split; eauto. repeat simpl_inject.
+  + generalize (RINJ r); rewrite Heqv; intro A; inv A.
+    rewrite Heqo.
+    eapply goto_label_inject; eauto. eapply globinj_to_funinj. auto.
+    repeat simpl_inject.
+Qed.
+
+Lemma allocframe_inject:
+  forall j stkb m0 m m1 m2 m3 m4 m' id path rs rs' sz ofs_link ofs_ra
+    (MS: match_states j (State rs m0) (State rs' m'))
+    (ALLOCF: Mem.alloc_frame m0 id = (m,path))
+    (ALLOC: Mem.alloc m 0 sz = (m1, stkb))
+    (SIZE: sz > 0)
+    (RECORDFR: Mem.record_frame (Mem.push_stage m1) (Memory.mk_frame sz) = Some m2)
+    (LINKPOS: 0 <= ofs_link <= Ptrofs.max_unsigned)
+    (STORELINK: Mem.store Mptr m2 stkb ofs_link (rs RSP) = Some m3 )
+    (RAPOS: 0 <= ofs_ra <= Ptrofs.max_unsigned)
+    (STORERA: Mem.store Mptr m3 stkb ofs_ra (rs RA) = Some m4 ),
+    let rs1 := (nextinstr (rs # RAX <- (rs RSP)) # RSP <- (Vptr stkb Ptrofs.zero)) in
+    let rs1' := (nextinstr (rs' # RAX <- (rs' RSP)) # RSP <- (Val.offset_ptr (rs' RSP) (Ptrofs.neg (Ptrofs.repr (align sz 8))))) in
+    exists j', inject_incr j j' /\
+    exists m1', Mem.storev Mptr m' (Val.offset_ptr (Val.offset_ptr (rs' RSP) (Ptrofs.neg (Ptrofs.repr (align sz 8)))) (Ptrofs.repr ofs_link)) (rs' RSP) = Some m1' /\
+    exists m2', Mem.storev Mptr m1' (Val.offset_ptr (Val.offset_ptr (rs' RSP) (Ptrofs.neg (Ptrofs.repr (align sz 8)))) (Ptrofs.repr ofs_ra)) (rs' RA)= Some m2' /\
+    match_states j' (State rs1 m4) (State rs1' m2').
+Proof.
+  intros.
+  inv MS. destruct RSPINJ' as [stkofs [Heqstkofs RSPINJ']].
+  remember (Ptrofs.unsigned stkofs) as stksize.
+  remember (align sz 8) as aligned_sz.
+  remember (stksize - aligned_sz) as stksize'.
+  exploit Mem.alloc_frame_left_inject; eauto. intro MINJ'.
+  (* reuse alloc_inject lemmas in memory *)
+  generalize (Mem.alloc_left_mapped_inject _ _ _ _ _ _ _ _ stksize' MINJ' ALLOC STKVB).
+  (* assert some properties about stack size *)
+  assert (ALGIN_SZ_ORDER: sz <= align sz 8). apply align_le. lia.
+  remember (Memory.mk_frame sz) as fr.
+  assert (FRSZ: sz = Memory.frame_size fr). rewrite Heqfr. simpl. lia.
+  assert (OLDSTKSIZE: aligned_sz <= stksize <= Ptrofs.max_unsigned).
+  {
+    split.
+    - rewrite Heqstkofs. apply Z.le_add_le_sub_r.
+      rewrite Heqaligned_sz. rewrite FRSZ.
+      remember (Mem.push_stage m1) as m1'.
+      generalize (Mem.record_frame_size1 m1' m2 fr RECORDFR). intros.
+      exploit Mem.support_push_stage. symmetry in Heqm1'.
+      apply Heqm1'. intros SUPPUSH. rewrite SUPPUSH in H.
+      simpl in H. unfold frame_size_a in H.
+      exploit Mem.astack_alloc. apply ALLOC. intros ALLOCSTK.
+      apply Mem.astack_alloc_frame in ALLOCF. rewrite ALLOCF.
+      rewrite <- ALLOCSTK. lia.
+    - rewrite Heqstksize. apply Ptrofs.unsigned_range_2.
+  }
+  assert (NEWSTKSIZE: 0 <= stksize' <= Ptrofs.max_unsigned).
+  {
+    rewrite Heqstksize'. rewrite Heqstksize.
+    split. lia.
+    lia.
+  }
+  (* prove for its premise *)
+  intro A.
+  trim A. lia.
+  trim A. intros. right. eapply STKPERMOFS. eauto.
+  trim A.
+  {
+    intros. eapply STKPERMOFS.
+    split. rewrite Heqstksize'. lia.
+    rewrite Heqstksize'. rewrite Heqstksize.
+    eapply Z.lt_le_trans with stksize. lia.
+    rewrite Heqstkofs.
+    generalize (Memory.stack_size_pos (Mem.astack (Mem.support m))).
+    intros STKSZPOS.
+    erewrite Mem.astack_alloc_frame; eauto.
+    lia.
+  }
+  trim A.
+  {
+    red. intros. subst.
+    eapply Z.divide_trans with 8.
+    destruct chunk; try (exists 8; reflexivity);
+      try (exists 4; reflexivity);
+      try (exists 2; reflexivity);
+      try (exists 1; reflexivity).
+    apply Z.divide_sub_r.
+    generalize (stack_size_aligned (Mem.astack (Mem.support m))).
+    intro ALI1.
+    assert (ALI2: (8 | Memory.max_stacksize)). unfold Memory.max_stacksize. red. exists 512. lia.
+    rewrite Heqstkofs.
+    apply Z.divide_sub_r; auto.
+    erewrite Mem.astack_alloc_frame; eauto.
+    apply align_divides. lia.
+  }
+  trim A.
+  {
+    intros b0 delta' ofs k p JB PERM OVERLAP.
+    subst. simpl in OVERLAP.
+    erewrite <- Mem.perm_alloc_frame in PERM; eauto.
+    generalize (STKINJLWBD _ _ _ _ _ JB PERM).
+    rewrite <- Heqstkofs. lia.
+  }
+  destruct A as (f1 & MINJ1 & INCR & EQ1 & EQ2).
+  exists f1. split. auto.
+  generalize (Mem.push_stage_left_inject _ _ _ MINJ1). intros MINJ2.
+  generalize (Mem.record_frame_left_inject _ _ _ _ _ MINJ2 RECORDFR). intros MINJ3.
+  (* store link *)
+  assert (ALIGNED_SZ: 0 <= align sz 8 <= Ptrofs.max_unsigned). lia.
+  exploit Mem.store_mapped_inject.
+  apply MINJ3. apply STORELINK. apply EQ1.
+  eapply val_inject_incr; eauto.
+  intros (m3' & STORELINK' & MINJ1').
+  exists m3'. split. subst.
+  rewrite RSPINJ'. simpl.
+  assert ((Ptrofs.add stkofs (Ptrofs.neg (Ptrofs.repr (align sz 8)))) = Ptrofs.repr (Ptrofs.unsigned stkofs - align sz 8)).
+  {
+    rewrite <- Ptrofs.sub_add_opp. unfold Ptrofs.sub.
+    rewrite (Ptrofs.unsigned_repr _ ALIGNED_SZ). reflexivity.
+  }
+  rewrite H. remember (Ptrofs.repr ofs_link) as OFS.
+  remember (Ptrofs.unsigned stkofs - align sz 8) as STKSIZE.
+  rewrite Ptrofs.add_commut.
+  assert (Ptrofs.unsigned (Ptrofs.add OFS (Ptrofs.repr STKSIZE)) =
+          Ptrofs.unsigned OFS + STKSIZE) as EQ'.
+  {
+    eapply Mem.address_inject; eauto.
+    exploit Mem.store_valid_access_3. exact STORELINK.
+    intro VA; eapply Mem.store_valid_access_1 in VA; eauto.
+    destruct VA. eapply H0.
+    rewrite HeqOFS. rewrite Ptrofs.unsigned_repr; generalize (size_chunk_pos Mptr); lia.
+  }
+  rewrite EQ'. rewrite HeqOFS.
+  rewrite (Ptrofs.unsigned_repr _ LINKPOS).
+  rewrite <- RSPINJ'. auto.
+  (* store ra *)
+  exploit Mem.store_mapped_inject.
+  apply MINJ1'. apply STORERA. apply EQ1.
+  eapply val_inject_incr; eauto.
+  intros (m4' & STORERA' & MINJ2').
+  exists m4'. split. subst.
+  rewrite RSPINJ'. simpl.
+  assert ((Ptrofs.add stkofs (Ptrofs.neg (Ptrofs.repr (align sz 8)))) = Ptrofs.repr (Ptrofs.unsigned stkofs - align sz 8)).
+  {
+    rewrite <- Ptrofs.sub_add_opp. unfold Ptrofs.sub.
+    rewrite (Ptrofs.unsigned_repr _ ALIGNED_SZ). reflexivity.
+  }
+  rewrite H. remember (Ptrofs.repr ofs_ra) as OFS.
+  remember (Ptrofs.unsigned stkofs - align sz 8) as STKSIZE.
+  rewrite Ptrofs.add_commut.
+  assert (Ptrofs.unsigned (Ptrofs.add OFS (Ptrofs.repr STKSIZE)) =
+          Ptrofs.unsigned OFS + STKSIZE) as EQ'.
+  {
+    eapply Mem.address_inject; eauto.
+    exploit Mem.store_valid_access_3. exact STORERA.
+    intro VA; eapply Mem.store_valid_access_1 in VA; eauto.
+    destruct VA. eapply H0.
+    rewrite HeqOFS. rewrite Ptrofs.unsigned_repr; generalize (size_chunk_pos Mptr); lia.
+  }
+  rewrite EQ'. rewrite HeqOFS.
+  rewrite (Ptrofs.unsigned_repr _ RAPOS). auto.
+  (* match state *)
+  assert (SUPINCALL: Mem.sup_include (Mem.support m0) (Mem.support m4)).
+  {
+    generalize (Mem.sup_include_alloc _ _ _ _ _ ALLOC).
+    remember (Mem.push_stage m1) as m1x. symmetry in Heqm1x.
+    generalize (Mem.sup_include_record_frame _ _ _ RECORDFR).
+    generalize (Mem.support_store _ _ _ _ _ _ STORELINK).
+    generalize (Mem.support_store _ _ _ _ _ _ STORERA).
+    intros.
+    eapply Mem.sup_include_trans.
+    intro. eapply Mem.support_alloc_frame_1 in ALLOCF. apply ALLOCF.
+    eapply Mem.sup_include_trans. apply H2.
+    rewrite H,H0.
+    eapply Mem.sup_include_trans. 2: apply H1.
+    inv Heqm1x. auto. simpl. unfold Mem.sup_push_stage.
+    intro. destruct b; simpl; auto.
+  }
+
+  assert (SUPINCALL': Mem.sup_include (Mem.support m') (Mem.support m4')).
+  {
+    generalize (Mem.support_store _ _ _ _ _ _ STORELINK').
+    generalize (Mem.support_store _ _ _ _ _ _ STORERA').
+    intros. rewrite H,H0. apply Mem.sup_include_refl.
+  }
+  remember (Ptrofs.repr stksize') as stkofs'.
+  assert(STKOFS': Ptrofs.unsigned stkofs' = Memory.max_stacksize - Memory.stack_size (Mem.astack (Mem.support m4))).
+  {
+    generalize (Mem.support_store _ _ _ _ _ _ STORELINK).
+    intro SUPSTLINK.
+    generalize (Mem.support_store _ _ _ _ _ _ STORERA).
+    intro SUPSTRA.
+    rewrite SUPSTRA,SUPSTLINK.
+    remember (Mem.push_stage m1) as m1x.
+    generalize (Mem.astack_record_frame _ _ _ RECORDFR).
+    intro SUPRDFR. destruct SUPRDFR as (hd & tl & (H1 & H2)).
+    symmetry in Heqm1x.
+    generalize (Mem.support_push_stage _ _ Heqm1x).
+    intro SUPPHST.
+    rewrite SUPPHST in H1. simpl in H1.
+    inversion H1. subst hd. clear H1.
+    generalize (Mem.astack_alloc _ _ _ _ _ ALLOC).
+    intro SUPAL. rewrite SUPAL in H3. simpl in H3.
+    rewrite <- H3 in H2.
+    rewrite H2.
+    assert (Memory.stack_size ((fr :: nil) :: Mem.astack (Mem.support m)) = (Memory.frame_size_a fr)+ Memory.stack_size (Mem.astack (Mem.support m))).
+    simpl. lia.
+    rewrite H. rewrite Heqstkofs'.
+    rewrite (Ptrofs.unsigned_repr _ NEWSTKSIZE).
+    rewrite Heqstksize'. rewrite Heqstkofs.
+    subst aligned_sz. unfold frame_size_a.
+    erewrite Mem.astack_alloc_frame; eauto.
+    rewrite FRSZ. lia.
+  }
+  econstructor; eauto.
+  (* Memory Injection *)
+  - constructor; eauto.
+    ++ intros. exploit defs_inject; eauto.
+    ++ intros until 0. intros JB' FD.
+       destruct (j b) eqn:JB1. destruct p.
+       exploit INCR; eauto. rewrite JB'; intro X. inv X.
+       exploit defs_rev_inject; eauto.
+       destruct (eq_block b stkb).
+       +++ subst. rewrite EQ1 in JB'. inv JB'.
+           apply Genv.genv_defs_range in FD. unfold stkblock in FD.
+           generalize (freshness (Genv.genv_sup ge)).
+           congruence.
+       +++ apply EQ2 in n. rewrite <- n in JB1.
+           rewrite JB1 in JB'. congruence.
+    ++ intros. exploit symbol_inject; eauto.
+  - eapply Mem.sup_include_trans. apply ENVSUP. auto.
+  - eapply Mem.sup_include_trans. apply ENVSUP'. auto.
+  (* Regset Injection *)
+  - intros. unfold rs1, rs1'.
+    apply val_inject_nextinstr; auto.
+    apply val_inject_set; auto.
+    apply val_inject_set; auto.
+    intros. eapply val_inject_incr; eauto.
+    eapply val_inject_incr; eauto.
+    rewrite RSPINJ'. econstructor; eauto.
+    subst.
+    rewrite Ptrofs.add_zero_l.
+    rewrite <- Ptrofs.sub_add_opp. unfold Ptrofs.sub.
+    rewrite Ptrofs.unsigned_repr; auto.
+  (* Stack Injection *)
+  - unfold Mem.valid_block. apply SUPINCALL'. auto.
+  - constructor.
+    intros ofs k p PERM.
+    apply (Mem.perm_store_2 _ _ _ _ _ _ STORERA') in PERM.
+    apply (Mem.perm_store_2 _ _ _ _ _ _ STORELINK') in PERM.
+    apply STKPERMOFS in PERM. auto.
+    intros ofs k p PERM.
+    eapply (Mem.perm_store_1 _ _ _ _ _ _ STORERA').
+    apply (Mem.perm_store_1 _ _ _ _ _ _ STORELINK').
+    apply STKPERMOFS. auto.
+  - unfold rs1. rewrite nextinstr_rsp, Pregmap.gss. eauto.
+  - exists stkofs'.
+    split. auto.
+    unfold rs1'. rewrite nextinstr_rsp. rewrite Pregmap.gss.
+    rewrite RSPINJ'. simpl.
+    assert (stkofs' =  (Ptrofs.add stkofs (Ptrofs.neg (Ptrofs.repr aligned_sz)))).
+    {
+      rewrite <- Ptrofs.sub_add_opp.
+      unfold Ptrofs.sub.
+      rewrite Heqstkofs'.
+      subst stksize'. subst stksize. subst aligned_sz.
+      rewrite (Ptrofs.unsigned_repr _ ALIGNED_SZ). reflexivity.
+    }
+    rewrite H. auto.
+  - red. intros b0 delta o k p JB PERM.
+    apply (Mem.perm_store_2 _ _ _ _ _ _ STORERA) in PERM.
+    apply (Mem.perm_store_2 _ _ _ _ _ _ STORELINK) in PERM.
+    remember (Mem.push_stage m1) as m1x.
+    apply (Mem.perm_record_frame _ _ _ RECORDFR) in PERM.
+    symmetry in Heqm1x.
+    apply (Mem.perm_push_stage _ _ Heqm1x) in PERM.
+    apply (Mem.perm_alloc_inv _ _ _ _ _ ALLOC) in PERM.
+    destruct eq_block.
+    * subst b0. rewrite EQ1 in JB.
+      inversion JB. subst delta. clear JB.
+      rewrite <- STKOFS'. rewrite Heqstkofs'.
+      rewrite (Ptrofs.unsigned_repr _ NEWSTKSIZE). lia.
+    * rewrite <- STKOFS'.
+      transitivity (Ptrofs.unsigned stkofs).
+      ** rewrite Heqstkofs'.
+         rewrite <- Heqstksize.
+         rewrite (Ptrofs.unsigned_repr _ NEWSTKSIZE). lia.
+      ** rewrite EQ2 in JB; auto.
+         unfold stack_inject_lowbound in STKINJLWBD.
+         rewrite <- Heqstkofs in STKINJLWBD.
+         rewrite Heqstksize in STKINJLWBD.
+         eapply STKINJLWBD; eauto.
+         eapply Mem.perm_alloc_frame; eauto.
+Qed.
+
+Lemma exec_instr_inject:
+  forall j m m' rs rs' f i m1 rs1
+    (EI: Asm.exec_instr ge f i rs m = Next rs1 m1)
+    (MS: match_states j (State rs m) (State rs' m'))
+    (AINR: asm_instr_unchange_rsp i)
+    (AINS: asm_instr_unchange_stk i),
+  exists j' m1' rs1',
+    exec_instr ge f i rs' m' = Next rs1' m1'
+    /\ match_states j' (State rs1 m1) (State rs1' m1')
+    /\ inject_incr j j'.
+Proof.
+  intros.
+  destruct (stk_unrelated_instr i) eqn:NOTSTKINSTR.
+  (* Normal Instructions *)
+  - (* Comment for speed *)
+    admit.
+(*
+    inversion MS.
+    edestruct exec_instr_inject_normal as (rs1' & m1' & EI' & MINJ' & RINJ'); eauto.
+    exists j, m1', rs1'; split; [|split]; eauto.
+    destruct i; simpl in *; eauto; try congruence.
+    subst.
+    generalize (asm_prog_unchange_support i). intro AIUS. red in AIUS.
+    edestruct (AINS NOTSTKINSTR _ _ _ _ _ _ EI) as (STACKEQ & STKPERMEQ).
+    edestruct (AINS NOTSTKINSTR _ _ _ _ _ _ EI') as (STACKEQ' & STKPERMEQ').
+    eapply match_states_intro; eauto.
+     + apply AIUS in EI.
+      eapply Mem.sup_include_trans. apply ENVSUP. auto.
+     + apply AIUS in EI'.
+       eapply Mem.sup_include_trans. apply ENVSUP'. auto.
+     + apply AIUS in EI'.
+       unfold Mem.valid_block. apply EI'. auto.
+     + constructor.
+       ++ intros ofs k p PERM.
+          apply STKPERMEQ' in PERM.
+          apply STKPERMOFS in PERM. auto.
+       ++ intros ofs k p OFS.
+          apply STKPERMEQ'.
+          apply STKPERMOFS. auto.
+     + rewrite (AINR _ _ _ _ _ _ NOTSTKINSTR EI) in RSPINJ. auto.
+     + rewrite (AINR _ _ _ _ _ _ NOTSTKINSTR EI') in RSPINJ'.
+       rewrite <- STACKEQ. auto.
+     + rewrite <- STACKEQ.
+      red. intros. apply STKPERMEQ in H0.
+       eapply STKINJLWBD; eauto. *)
+  (* Specail Cases *)
+    Opaque Mem.alloc_frame.
+  - destruct i; simpl in *; try congruence.
+    (* Pcall_s *)
+    + destr_in EI. inv MS.
+      do 4 eexists. split. eauto. split. econstructor; eauto.
+      * intros. apply val_inject_set. auto.
+        intros. apply val_inject_set. auto.
+        apply Val.offset_ptr_inject. auto.
+        destruct Genv.symbol_address eqn: SYMBBLOCK; eauto.
+        unfold Genv.symbol_address in SYMBBLOCK.
+        destruct Genv.find_symbol eqn: FS in SYMBBLOCK; inv SYMBBLOCK.
+        exploit symbol_inject. apply GLOBINJ. apply FS. intros.
+        apply (Val.inject_ptr j b Ptrofs.zero b Ptrofs.zero 0); eauto.
+      * red. auto.
+    (* Pcall_r *)
+    + destr_in EI. inv MS.
+      do 4 eexists. split. eauto. split. econstructor; eauto.
+      * intros. apply val_inject_set. auto.
+        intros. apply val_inject_set. auto.
+        apply Val.offset_ptr_inject. auto.
+        eauto.
+      * red. auto.
+    (* Pret *)
+    + destr_in EI. inv MS.
+      do 4 eexists. split. eauto. split. econstructor; eauto.
+      * intros. apply val_inject_set. auto.
+        intros. auto.
+      * red. auto.
+    (* Pallocframe *)
+    + repeat destr_in EI.
+      inversion MS. subst.
+      edestruct allocframe_inject as (j' & INCR & m1' & STORERA & m2' & STORELINK & MS') ; eauto. admit.
+      apply Ptrofs.unsigned_range_2.
+      apply Ptrofs.unsigned_range_2.
+      rewrite Ptrofs.repr_unsigned in STORERA.
+      rewrite Ptrofs.add_zero_l in STORERA.
+      rewrite Ptrofs.repr_unsigned in STORELINK.
+      rewrite Ptrofs.add_zero_l in STORELINK.
+      rewrite STORERA. rewrite STORELINK.
+      eexists j',_,_; split; eauto.
+    (* Pfreeframe *)
+    + repeat destr_in EI.
+      rename Heqv1 into RSRSP.
+      rename Heqo into LOADRA.
+      rename Heqo0 into LOADLINK.
+      rename Heqo1 into FREE.
+      rename Heqo2 into RET.
+      rename Heqo3 into POP.
+      inv MS. rewrite RSRSP in RSPINJ.
+      destruct RSPINJ as [tmp EQ]. inversion EQ.
+      symmetry in H0. subst. clear EQ.
+      clear NOTSTKINSTR.
+      rename v into val_ra.
+      rename v0 into val_link.
+      exploit Mem.loadv_inject. apply MINJ. apply LOADRA.
+      apply Val.offset_ptr_inject. rewrite <- RSRSP. auto.
+      intros (val_ra' & LOADRA' & INJRA). rewrite LOADRA'.
+      exploit Mem.loadv_inject. apply MINJ. apply LOADLINK.
+      apply Val.offset_ptr_inject. rewrite <- RSRSP. auto.
+      intros (val_link' & LOADLINK' & INJLINK). rewrite LOADLINK'.
+      exists j; eexists; eexists; split; [|split]; eauto.
+      constructor; eauto.
+      (* Memory Injection *)
+      * eapply Mem.pop_stage_left_inject. 2: eauto.
+        eapply Mem.return_frame_left_inject. 2: eauto.
+        eapply Mem.free_left_inject; eauto.
+      * apply Mem.support_free in FREE.
+        apply Mem.sup_include_pop_stage in POP.
+        rewrite <- FREE in ENVSUP.
+        eapply Mem.sup_include_trans. apply ENVSUP.
+        eapply Mem.sup_include_trans. 2 : eauto.
+        intro. eapply Mem.support_return_frame_1 in RET. apply RET.
+      (* Regset Injection *)
+      * intros; apply val_inject_nextinstr.
+        intros; apply val_inject_set; auto.
+        intros; apply val_inject_set; auto.
+      (* Stack Injection *)
+      * rewrite nextinstr_rsp.
+        rewrite Pregmap.gso by congruence.
+        rewrite Pregmap.gss.
+        (* Goal: exists b0 : block, val_link = Vptr b0 Ptrofs.zero *)
+        (* val_link is its parent rsp *)
+        (* (parent_sp (Mem.stack m)) *)
+        admit.
+      * rewrite nextinstr_rsp.
+        rewrite ! Pregmap.gso by congruence.
+        rewrite Pregmap.gss.
+        (* Goal: exists b0 : block, val_link = Vptr b0 Ptrofs.zero *)
+        (* val_link is its parent rsp *)
+        (* (parent_sp (Mem.stack m)) *)
+        admit.
+Admitted.
+
+(* injection in builtin *)
+Lemma eval_builtin_arg_inject:
+  forall (rs:regset) sp m j (rs':regset) sp' m' a v
+    (SPINJ: Val.inject j sp sp')
+    (RINJ: forall r, Val.inject j rs#r rs'#r)
+    (MINJ: Mem.inject j m m')
+    (GLOBINJ: meminj_preserves_globals j),
+    eval_builtin_arg ge (fun r => rs#r) sp m a v ->
+    exists v', eval_builtin_arg ge (fun r => rs'#r) sp' m' a v' /\ Val.inject j v v'.
+Proof.
+  intros until 4.
+  induction 1.
+- exists (rs'#x); auto with barg.
+- econstructor; eauto with barg.
+- econstructor; eauto with barg.
+- econstructor; eauto with barg.
+- econstructor; eauto with barg.
+- exploit Mem.loadv_inject; eauto. apply Val.offset_ptr_inject. eauto.
+  intros (v' & P & Q). exists v'; eauto with barg.
+- econstructor; split; eauto with barg.
+  apply Val.offset_ptr_inject; eauto.
+- assert (Val.inject j (Senv.symbol_address ge id ofs) (Senv.symbol_address ge id ofs)).
+  { unfold Senv.symbol_address; simpl; unfold Genv.symbol_address.
+    destruct (Genv.find_symbol ge id) as [b|] eqn:FS; auto.
+    exploit symbol_inject; eauto. intros.
+    econstructor; eauto. rewrite Ptrofs.add_zero; auto. }
+  exploit Mem.loadv_inject; eauto.
+  intros (v' & A & B). exists v'; auto with barg.
+- econstructor; split; eauto with barg.
+  unfold Senv.symbol_address; simpl; unfold Genv.symbol_address.
+  destruct (Genv.find_symbol ge id) as [b|] eqn:FS; auto.
+  exploit symbol_inject; eauto. intros.
+  econstructor; eauto. rewrite Ptrofs.add_zero; auto.
+- destruct IHeval_builtin_arg1 as (v1' & A1 & B1); eauto using in_or_app.
+  destruct IHeval_builtin_arg2 as (v2' & A2 & B2); eauto using in_or_app.
+  exists (Val.longofwords v1' v2'); split; auto with barg.
+  apply Val.longofwords_inject; auto.
+- destruct IHeval_builtin_arg1 as (v1' & A1 & B1); eauto using in_or_app.
+  destruct IHeval_builtin_arg2 as (v2' & A2 & B2); eauto using in_or_app.
+  econstructor; split; eauto with barg.
+  destruct Archi.ptr64; auto using Val.add_inject, Val.addl_inject.
+Qed.
+
+Lemma eval_builtin_args_inject:
+  forall (rs:regset) sp m j (rs':regset) sp' m' al vl
+    (SPINJ: Val.inject j sp sp')
+    (RINJ: forall r, Val.inject j rs#r rs'#r)
+    (MINJ: Mem.inject j m m')
+    (GLOBINJ: meminj_preserves_globals j),
+    eval_builtin_args ge rs sp m al vl ->
+    exists vl', eval_builtin_args ge rs' sp' m' al vl' /\  Val.inject_list j vl vl'.
+Proof.
+  intros until 4.
+  induction 1; intros.
+- exists (@nil val); split; constructor.
+- exploit eval_builtin_arg_inject; eauto using in_or_app. intros (v1' & A & B).
+  destruct IHlist_forall2 as (vl' & C & D); eauto using in_or_app.
+  exists (v1' :: vl'); split; constructor; auto.
+Qed.
+
+(** injection in extcall *)
+Lemma extcall_arg_inject:
+  forall j rs1 m1 arg1 loc rs2 m2,
+    extcall_arg rs1 m1 loc arg1 ->
+    (forall r, Val.inject j (rs1 r) (rs2 r)) ->
+    Mem.inject j m1 m2 ->
+    exists arg2,
+      extcall_arg rs2 m2 loc arg2 /\
+      Val.inject j arg1 arg2.
+Proof.
+  destruct 1; simpl; intros.
+  eexists; split; try econstructor; eauto.
+  exploit Mem.loadv_inject; eauto.
+  apply Val.offset_ptr_inject; eauto.
+  intros (v2 & LOAD & INJ).
+  eexists; split; try econstructor; eauto.
+Qed.
+
+Lemma extcall_arg_pair_inject:
+  forall j rs1 m1 arg1 ty rs2 m2,
+    extcall_arg_pair rs1 m1 ty arg1 ->
+    (forall r, Val.inject j (rs1 r) (rs2 r)) ->
+    Mem.inject j m1 m2 ->
+    exists arg2,
+      extcall_arg_pair rs2 m2 ty arg2 /\
+      Val.inject j arg1 arg2.
+Proof.
+  destruct 1; simpl; intros.
+  eapply extcall_arg_inject in H; eauto.
+  destruct H as (arg2 & EA & INJ);
+    eexists; split; try econstructor; eauto.
+  eapply extcall_arg_inject in H; eauto.
+  destruct H as (arg2 & EA & INJ).
+  eapply extcall_arg_inject in H0; eauto.
+  destruct H0 as (arg3 & EA1 & INJ1).
+  eexists; split; try econstructor; eauto.
+  apply Val.longofwords_inject; eauto.
+Qed.
+
+Lemma extcall_arguments_inject:
+  forall j rs1 m1 args1 sg rs2 m2,
+    extcall_arguments rs1 m1 sg args1 ->
+    (forall r, Val.inject j (rs1 r) (rs2 r)) ->
+    Mem.inject j m1 m2 ->
+    exists args2,
+      extcall_arguments rs2 m2 sg args2 /\
+      Val.inject_list j args1 args2.
+Proof.
+  unfold extcall_arguments.
+  intros j rs1 m1 args1 sg rs2 m2.
+  revert args1. generalize (Conventions1.loc_arguments sg).
+  induction 1; simpl; intros; eauto.
+  exists nil; split; try econstructor.
+  eapply extcall_arg_pair_inject in H; eauto.
+  decompose [ex and] H.
+  edestruct IHlist_forall2 as (a2 & EA & INJ); eauto.
+  eexists; split; econstructor; eauto.
+Qed.
+
+(** Step Simulation *)
+Theorem step_simulation:
+  forall S1 t S2,
+    Asm.step ge S1 t S2 ->
+    forall j S1' (MS: match_states j S1 S1'),
+    exists j' S2',
+      step ge S1' t S2' /\
+      match_states j' S2 S2'.
+Proof.
+  destruct 1; intros; inversion MS; subst.
+  - (* internal step *)
+    generalize (RINJ PC); rewrite H. inversion 1; subst.
+    generalize (globinj_to_funinj j GLOBINJ). intros GLOBFUN_INJ.
+    assert (j b = Some (b,0)) as JB.
+    {
+      eapply GLOBFUN_INJ. eauto.
+    }
+    rewrite JB in H7; inv H7.
+    assert (asm_instr_unchange_rsp i).
+    {
+      eapply prog_unchange_rsp; eauto.
+    }
+    destruct (exec_instr_inject _ _ _ _ _ _ _ _ _ H2 MS H4 (asm_prog_unchange_stk i)) as ( j' & rs2' & m2' & EI' & MS' & INCR).
+    do 2 eexists; split.
+    eapply exec_step_internal; eauto.
+    rewrite Ptrofs.add_zero. eauto.
+    eauto.
+  - (* builtin step *)
+    edestruct (eval_builtin_args_inject) as (vargs' & Hargs & Hargsinj); eauto.
+    edestruct (external_call_mem_inject_gen ef)
+      as (j' & vres' & m2' & EC & RESinj & MemInj & Unch1 & Unch2 & INCR & SEP); try eauto. apply globals_symbols_inject. eauto.
+    exploit (external_call_astack ef). apply H3. intros STKEQ.
+    exploit (external_call_astack ef). apply EC. intros STKEQ0.
+    generalize (globinj_to_funinj j GLOBINJ). intros GLOBFUN_INJ.
+    assert (j b = Some (b,0)) as JB.
+    {
+      eapply GLOBFUN_INJ. eauto.
+    }
+    generalize (RINJ PC); rewrite H. inversion 1; subst.
+    rewrite JB in H8; inv H8.
+    do 2 eexists; split.
+    eapply exec_step_builtin; eauto.
+    rewrite Ptrofs.add_zero; eauto.
+    generalize (Mem.unchanged_on_support (loc_unmapped j) m m' Unch1).
+    intro SUPINCMEM.
+    generalize (Mem.unchanged_on_support (loc_out_of_reach j m) m'0 m2' Unch2).
+    intro SUPINCMEM1.
+    econstructor; eauto.
+    (* Memory Injection *)
+    + constructor.
+      ++ intros. exploit defs_inject; eauto.
+      ++ intros until 0. intros JB' FD.
+         destruct (j b) eqn:JB1. destruct p.
+         exploit INCR; eauto. rewrite JB'; intro X. inv X.
+         exploit defs_rev_inject; eauto.
+         exploit SEP; eauto.
+         unfold Mem.valid_block.
+         intros (NV1 & NV2).
+         exploit Genv.genv_defs_range. apply FD. intros.
+         apply ENVSUP' in H5. congruence.
+      ++ intros. exploit symbol_inject; eauto.
+    + eapply Mem.sup_include_trans. apply ENVSUP. auto.
+    + eapply Mem.sup_include_trans. apply ENVSUP'. auto.
+    (* Regset Injection *)
+    + intros. apply val_inject_nextinstr_nf.
+      apply val_inject_set_res; auto.
+      apply val_inject_undef_regs; auto.
+      intros; eapply val_inject_incr; eauto.
+    (* Stack Injection *)
+    + unfold Mem.valid_block. apply SUPINCMEM1. auto.
+    + constructor.
+      ++ intros ofs0 k p PERM.
+         (* Goal: Mem.perm m2' stkblock ofs0 k p =>
+            0 <= ofs0 < Ptrofs.max_unsigned *)
+         (* add new external call property *)
+         (*
+              ec_perm_frames:
+                forall ge args m1 t res m2,
+                  sem ge args m1 t res m2 ->
+                  forall b o k p,
+                      in_stack (Mem.stack m1) b ->
+                      Mem.perm m2 b o k p <-> Mem.perm m1 b o k p;
+          *)
+         admit.
+      ++ intros.
+         (* add new external call property *)
+         admit.
+    + remember (nextinstr_nf (set_res res vres (undef_regs (map preg_of (Machregs.destroyed_by_builtin ef)) rs))) as rs'.
+      destruct prog_unchange_rsp as (INT & BUILTIN & EXTCALL).
+      red in BUILTIN.
+      destruct (BUILTIN b2 ofs f ef args res rs m vargs t vres rs' m'); eauto.
+    + remember (nextinstr_nf (set_res res vres' (undef_regs (map preg_of (Machregs.destroyed_by_builtin ef)) rs'0))) as rs'.
+      destruct prog_unchange_rsp as (INT & BUILTIN & EXTCALL).
+      red in BUILTIN.
+      destruct (BUILTIN b2 ofs f ef args res rs'0 m'0 vargs' t vres' rs' m2'); eauto.
+      rewrite <- STKEQ. auto.
+    + red. intros b delta o k p JB1' PERM.
+      assert (JB1: j b = Some (stkblock, delta)).
+      {
+        destruct (j b) eqn:JB1. destruct p0.
+        - apply INCR in JB1. rewrite JB1 in JB1'. auto.
+        - exploit SEP. apply JB1. apply JB1'.
+          intros (NVB1 & NVB2). congruence.
+      }
+      rewrite <- STKEQ.
+      red in STKINJLWBD. eapply STKINJLWBD.
+      red in INCR.
+      apply JB1.
+      eapply Mem.perm_max in PERM.
+      eapply external_call_max_perm; eauto.
+      eapply Mem.valid_block_inject_1; eauto.
+  - (* external call *)
+    edestruct (extcall_arguments_inject) as (vargs' & Hargs & Hargsinj); eauto.
+    edestruct (external_call_mem_inject_gen ef) as (j' & vres' & m2' & EC & RESinj & MemInj & Unch1 & Unch2 & INCR & SEP); try eauto. apply globals_symbols_inject. eauto.
+    exploit (external_call_astack ef). apply H2. intros STKEQ.
+    exploit (external_call_astack ef). apply EC. intros STKEQ0.
+    generalize (RINJ PC); rewrite H.
+    intro VINJ; inv VINJ. rename H6 into JB2. rename H5 into EQofs.
+    generalize (globinj_to_funinj j GLOBINJ). intros GLOBFUN_INJ.
+    assert (j b = Some (b,0)) as JB.
+    {
+      eapply GLOBFUN_INJ. eauto.
+    }
+    rewrite JB in JB2; inv JB2.
+    do 2 eexists; split.
+    eapply exec_step_external; eauto.
+    generalize (Mem.unchanged_on_support (loc_unmapped j) m m' Unch1).
+    intro SUPINCMEM.
+    generalize (Mem.unchanged_on_support (loc_out_of_reach j m) m'0 m2' Unch2).
+    intro SUPINCMEM1.
+    econstructor; eauto.
+    (* Memory Injection *)
+    + constructor.
+      ++ intros. exploit defs_inject; eauto.
+      ++ intros until 0. intros JB' FD.
+         destruct (j b) eqn:JB1. destruct p.
+         exploit INCR; eauto. rewrite JB'; intro X. inv X.
+         exploit defs_rev_inject; eauto.
+         exploit SEP; eauto.
+         unfold Mem.valid_block.
+         intros (NV1 & NV2).
+         exploit Genv.genv_defs_range. apply FD. intros.
+         apply ENVSUP' in H3. congruence.
+      ++ intros. exploit symbol_inject; eauto.
+    + eapply Mem.sup_include_trans. apply ENVSUP. auto.
+    + eapply Mem.sup_include_trans. apply ENVSUP'. auto.
+    (* Regset Injection *)
+    + intros; apply val_inject_set.
+      intros; apply val_inject_set_pair; auto.
+      apply val_inject_undef_caller_save_regs; auto.
+      intros; eapply val_inject_incr; eauto.
+      intros; eapply val_inject_incr; eauto.
+    (* Stack Injection *)
+    + unfold Mem.valid_block. apply SUPINCMEM1. auto.
+    + constructor.
+      ++ intros ofs0 k p PERM.
+         (* add new external call property *)
+         admit.
+      ++ intros.
+         (* add new external call property *)
+         admit.
+    + remember ((set_pair (loc_external_result (ef_sig ef)) res (undef_caller_save_regs rs)) # PC <- (rs RA)) as rs'.
+      destruct prog_unchange_rsp as (INT & BUILTIN & EXTCALL).
+      red in EXTCALL.
+      destruct (EXTCALL b2 ef args res rs m t rs' m'); eauto.
+    + remember ((set_pair (loc_external_result (ef_sig ef)) vres'
+     (undef_caller_save_regs rs'0)) # PC <- (rs'0 RA)) as rs'.
+      destruct prog_unchange_rsp as (INT & BUILTIN & EXTCALL).
+      red in EXTCALL.
+      destruct (EXTCALL b2 ef vargs' vres' rs'0 m'0 t rs' m2'); eauto.
+      rewrite <- STKEQ. eauto.
+    + red. intros b delta o k p JB1' PERM.
+      assert (JB1: j b = Some (stkblock, delta)).
+      {
+        destruct (j b) eqn:JB1. destruct p0.
+        - apply INCR in JB1. rewrite JB1 in JB1'. auto.
+        - exploit SEP. apply JB1. apply JB1'.
+          intros (NVB1 & NVB2). congruence.
+      }
+      rewrite <- STKEQ.
+      red in STKINJLWBD. eapply STKINJLWBD.
+      red in INCR.
+      apply JB1.
+      eapply Mem.perm_max in PERM.
+      eapply external_call_max_perm; eauto.
+      eapply Mem.valid_block_inject_1; eauto.
+Admitted.
+
+Lemma transf_initial_states:
+  forall st1, Asm.initial_state prog st1 ->
+  exists j st2, SSAsm.initial_state prog st2 /\ match_states j st1 st2.
+Proof.
+  inversion 1. subst.
+  rename H into INIT.
+  rename H0 into INITMEM.
+  exploit Genv.initmem_inject; eauto. intro FLATINJ.
+(*
+  assert (ALLOCINJ: exists (j : meminj) (m1' m2' : mem) (stk' : block),
+             Mem.alloc m0 0 Memory.max_stacksize = (m1', stk) /\
+             Mem.record_frame (Mem.push_stage m1') (Memory.mk_frame Memory.max_stacksize) = Some m2' /\
+             Mem.inject j m0 m2' /\
+             inject_incr (Mem.flat_inj (Mem.support m0)) j /\
+             j stk = Some (stk', Memory.max_stacksize) /\
+             (forall b : block, b <> stk -> j b = Mem.flat_inj (Mem.support m0) b)).
+  {
+    admit.
+  } *)
+ (* destruct ALLOCINJ as (j & m1' & m2' & stk' & ALLOC' & RECORDFR' & ALLOCINJ & INCR & INJSTK & INJDEF).
+  assert (stk' = stk).
+  {
+    admit.
+  } subst.
+  assert (stk = stkblock).
+  {
+    admit.
+  } subst.  
+  eexists j, _. split. *)
+  (* initial_state *)
+  caseEq (Mem.alloc m0 0 max_stacksize). intros.
+  assert ({m1|Mem.record_frame (Mem.push_stage m) (mk_frame max_stacksize) = Some m1}).
+  apply Mem.request_record_frame. simpl. congruence.
+  assert (Mem.astack (Mem.support (Mem.push_stage m)) = nil::nil).
+  exploit Genv.init_mem_astack; eauto. intro.
+  apply Mem.astack_alloc in H. simpl. rewrite H. rewrite H0. auto.
+  rewrite H0.
+  unfold max_stacksize. unfold frame_size_a. simpl.
+  unfold align. simpl. lia.
+  destruct X as (m1 & RECORD).
+  eexists (Mem.flat_inj (Mem.support m0)) ,_. split.
+  econstructor; eauto.
+  constructor; eauto.
+  eapply Mem.record_frame_right_inject. 2: eauto.
+  eapply Mem.push_stage_right_inject; eauto.
+  eapply Mem.alloc_right_inject; eauto.
+  admit. admit. admit.
+    + intros. unfold rs0.
+      repeat (intros; apply val_inject_set; auto). fold ge0.
+      admit. constructor. constructor.
+      ++ unfold ge0. unfold Genv.symbol_address.
+         destruct (Genv.find_symbol (Genv.globalenv prog) (prog_main prog)) eqn:E.
+         econstructor; eauto.
+         exploit Genv.genv_symb_range. eauto. intro.
+         erewrite INJDEF. unfold Mem.flat_inj.
+         rewrite pred_dec_true. eauto.
+
+         exploit Genv.init_mem_genv_sup; eauto. intro.
+         rewrite <- H0. auto.
+         unfold stkblock. unfold not. intro.
+         generalize (freshness (Genv.genv_sup ge)). intro.
+         rewrite H0 in H.  unfold ge in *. congruence.
+         unfold Vnullptr; constructor.
+         econstructor.
+  intros. destruct r. simpl. constructor.
+  Search meminj_preserves_globals.
+  Search Genv.init_mem.
+  - econstructor.
+    + apply INITMEM.
+    + apply ALLOC'.
+    + apply RECORDFR'.
+  (* match_state *)
+  - remember (Mem.push_stage m1) as m1x.
+    symmetry in Heqm1x.
+    exploit Genv.init_mem_genv_sup. apply INITMEM.
+    generalize (Mem.sup_include_alloc _ _ _ _ _ ALLOC).
+    generalize (Mem.sup_include_push_stage _ _ Heqm1x).
+    generalize (Mem.sup_include_record_frame _ _ _ RECORDFR).
+    intros SUPREC SUPPUSH SUPALLOC SUPINIT.
+    remember (Mem.push_stage m1') as m1x'.
+    symmetry in Heqm1x'.
+    generalize (Mem.sup_include_alloc _ _ _ _ _ ALLOC').
+    generalize (Mem.sup_include_push_stage _ _ Heqm1x').
+    generalize (Mem.sup_include_record_frame _ _ _ RECORDFR').
+    intros SUPREC' SUPPUSH' SUPALLOC'.
+    econstructor; eauto.
+    (* Memory Injection *)
+    + constructor; eauto.
+      ++ intros.
+         assert (sup_In b (Genv.genv_sup ge)).
+         {
+           unfold Genv.find_funct_ptr in H. repeat destr_in H.
+           eapply Genv.genv_defs_range in H1; eauto.
+         }
+         rewrite INJDEF. unfold Mem.flat_inj.
+         destruct (Mem.sup_dec b (Mem.support m0)). auto.
+         destruct n.
+         rewrite <- SUPINIT. unfold ge in H0. auto.
+         unfold stkblock. unfold not. intro.
+         generalize (freshness (Genv.genv_sup ge)). intro.
+         rewrite <- H1 in H2. congruence.
+      ++ intros.
+         rewrite INJDEF in H. unfold Mem.flat_inj in H.
+         destruct (Mem.sup_dec b (Mem.support m0)).
+         +++ inv H. auto.
+         +++ inv H.
+         +++ unfold not. intro.
+             rewrite H1 in H.
+             rewrite INJSTK in H. inv H.
+             eapply Genv.genv_defs_range in H0; eauto.
+             unfold stkblock in H0.
+             generalize (freshness (Genv.genv_sup ge)). intro.
+             congruence.
+      ++ intros.
+         unfold Genv.find_symbol in H.
+         exploit Genv.genv_symb_range. eauto. intro H1.
+         rewrite INJDEF. unfold Mem.flat_inj.
+         destruct (Mem.sup_dec b (Mem.support m0)). auto.
+         destruct n.
+         rewrite <- SUPINIT. unfold ge in H1. auto.
+         unfold stkblock. unfold not. intro.
+         generalize (freshness (Genv.genv_sup ge)). intro.
+         rewrite H0 in H1. congruence.
+    + exploit Genv.init_mem_genv_sup; eauto. intros.
+      rewrite <- H. unfold ge. apply Mem.sup_include_refl.
+    + unfold ge. rewrite SUPINIT.
+      eapply Mem.sup_include_trans. apply SUPALLOC'.
+      eapply Mem.sup_include_trans. apply SUPPUSH'.
+      eapply Mem.sup_include_trans. apply SUPREC'.
+      apply Mem.sup_include_refl.
+    (* Regset Injection *)
+    + intros. unfold rs0.
+      repeat (intros; apply val_inject_set; auto).
+      ++ unfold ge0. unfold Genv.symbol_address.
+         destruct (Genv.find_symbol (Genv.globalenv prog) (prog_main prog)) eqn:E.
+         econstructor; eauto.
+         exploit Genv.genv_symb_range. eauto. intro.
+         erewrite INJDEF. unfold Mem.flat_inj.
+         rewrite pred_dec_true. eauto.
+
+         exploit Genv.init_mem_genv_sup; eauto. intro.
+         rewrite <- H0. auto.
+         unfold stkblock. unfold not. intro.
+         generalize (freshness (Genv.genv_sup ge)). intro.
+         rewrite H0 in H.  unfold ge in *. congruence.
+         unfold Vnullptr; constructor.
+         econstructor.
+      ++ econstructor.
+      ++ econstructor. apply INJSTK. rewrite Ptrofs.add_zero_l. auto.
+    (* Stack Injection *)
+    + red. apply SUPREC', SUPPUSH'.
+      exploit Mem.nextblock_alloc; eauto. intro.
+      exploit Mem.support_alloc; eauto. intro.
+      rewrite H0. unfold stkblock.
+      unfold ge. rewrite SUPINIT.
+      unfold sup_incr.
+      eapply Mem.sup_add_in. left. auto.
+    + constructor.
+      ++ intros ofs k p PERM.
+         generalize (Mem.perm_record_frame _ _ _ RECORDFR'). intro.
+         generalize (Mem.perm_push_stage _ _ Heqm1x'). intro.
+         generalize (Mem.perm_alloc_inv _ _ _ _ _ ALLOC'). intro.
+         apply H,H0,H1 in PERM.
+         rewrite pred_dec_true in PERM; eauto.
+         assert (Mem.max_stacksize < Ptrofs.max_unsigned).
+         {
+           unfold Mem.max_stacksize.
+           vm_compute. auto.
+         }.
+         lia.
+      ++ intros.
+         generalize (Mem.perm_record_frame _ _ _ RECORDFR'). intro.
+         generalize (Mem.perm_push_stage _ _ Heqm1x'). intro.
+         generalize (Mem.perm_alloc_inv _ _ _ _ _ ALLOC'). intro.
+         apply H0, H1.
+Admitted.
+
+
+Lemma transf_final_states:
+  forall j st1 st2 r,
+    match_states j st1 st2 -> Asm.final_state st1 r -> final_state st2 r.
+Proof.
+    inversion 1; subst.
+    inversion 1; subst.
+    econstructor.
+    generalize (RINJ PC). rewrite H3. unfold Vnullptr. destruct Archi.ptr64; inversion 1; auto.
+    generalize (RINJ RAX). rewrite H5. unfold Vnullptr. destruct Archi.ptr64; inversion 1; auto.
+Qed.
+
+Theorem transf_program_correct:
+  forward_simulation (Asm.semantics prog) (SSAsm.semantics prog).
+Proof.
+  eapply forward_simulation_step with (fun s1 s2 => exists j o, match_states j s1 s2).
+  - simpl. reflexivity.
+  - simpl. intros s1 IS; inversion IS.
+    exploit transf_initial_states. eauto.
+    intros (j & st2 & MIS & MS); eexists; split; eauto. inv MIS. eauto.
+  - simpl. intros s1 s2 r (j & o & MS) FS. eapply transf_final_states; eauto.
+  - simpl. intros s1 t s1' STEP s2 (j & o & MS).
+    edestruct step_simulation as (j' & s2' & STEP' & MS'); eauto.
+Qed.
+
+End PRESERVATION.
